DDC/src/classes.v
@@ -1,0 +1,189 @@
+Require Import Metalib.Metatheory.
+Require Import Metalib.LibLNgen.
+
+Create HintDb syntax.
+Create HintDb fv.
+Create HintDb open.
+Create HintDb close.
+Create HintDb size.
+Create HintDb subst.
+Create HintDb lc.
+
+(***********************************************************************)
+(** * Operations *)
+(***********************************************************************)
+
+(* operations with a single type *)
+
+Class Syntax (e :  Set) := {
+    fv : e -> vars ;
+    lc : e -> Prop;
+    close_rec : nat -> atom -> e -> e ;
+    size : e -> nat;
+}.
+
+Definition close {e} `{ Syntax e} := close_rec 0.
+
+(* operations with multiple types *)
+
+Class Subst (e : Set) (u : Set) `{Syntax e} `{Syntax u} := {
+    open_rec  : nat -> u -> e -> e ;
+    subst : u -> atom -> e -> e    
+}.
+
+Definition open {e}{u} `{Subst e u}  (e0 : e) (u0 : u) := open_rec 0 u0 e0.
+
+(***********************************************************************)
+(** * Theory *)
+(***********************************************************************)
+
+(* These are the general form of the lemmas in the Lemmas.v file; and 
+   perhaps automatically proven by a future version of LNgen. *)
+   
+
+Class SyntaxTheory (exp : Set) `{H: Syntax exp} := {
+
+    fv_close : forall a1 x1,
+      fv (close x1 a1) [=] remove x1 (fv a1);
+    
+    close_inj : forall (e1 : exp) e2 x1,
+      close x1 e1 = close x1 e2 ->
+      e1 = e2;
+   }.
+
+
+Class SubstOpenTheory (exp : Set) (u : Set) (uvar : atom -> u) `{H: Subst exp u} 
+      `{HU: Subst u u} := {
+    
+    subst_open : forall (a3 : exp) (a1 : u) (a2 : u) x1,
+      lc a1 -> 
+      subst a1 x1 (open a3 a2) = open (subst a1 x1 a3) (subst a1 x1 a2);
+  }.
+
+Class SubstTheory (exp : Set) (u : Set) (uvar : atom -> u) `{H: Subst exp u} := {
+    
+    fv_open_lower : forall a1 a2,
+      fv a1 [<=] fv (open a1 a2);
+    
+    fv_open_upper : forall a1 a2,
+      fv (open a1 a2) [<=] fv a2 `union` fv a1;
+    
+    open_close : forall (e1 : exp) x1,
+      open (close x1 e1) (uvar x1) = e1;
+
+    size_open_var : forall a x, 
+      size (open a (uvar x)) = size a;
+    
+    open_inj : forall (e2 e1:exp) x1,
+      x1 `notin` fv e2 ->
+      x1 `notin` fv e1 ->
+      open e2 (uvar x1) = open e1 (uvar x1) ->
+      e2 = e1;
+
+    subst_intro  : forall (x1:atom) (e1 : exp) (e2 : u),
+      x1 `notin` fv e1 ->
+      open e1 e2  = subst e2 x1 (open e1 (uvar x1)) ;
+    
+    subst_open_var : forall (e2 : exp) e1 x1 x2,
+      x1 <> x2 ->
+      lc e1 ->
+      open (subst e1 x1 e2) (uvar x2) = 
+        subst e1 x1 (open e2 (uvar x2));
+    
+    subst_fresh_eq : forall a2 a1 x1,
+      x1 `notin` fv a2 ->
+      subst a1 x1 a2 = a2;
+        
+    subst_lc : forall a1 a2 x1,
+      lc a1 ->
+      lc a2 ->
+      lc (subst a2 x1 a1);
+    
+    subst_spec: forall a1 a2 x1, 
+      subst a2 x1 a1 = open (close x1 a1) a2;
+                                        
+    subst_close : forall a2 a1 x1 x2,
+      lc a1 ->  x1 <> x2 ->
+      x2 `notin` fv a1 ->
+      subst a1 x1 (close x2 a2) = close x2 (subst a1 x1 a2);
+
+  (* still not included 
+     
+  fv_subst_fresh := fv_exp_subst_exp_wrt_exp_fresh;
+  fv_subst_lower := fv_exp_subst_exp_wrt_exp_lower;
+  fv_subst_notin := fv_exp_subst_exp_wrt_exp_notin;
+  fv_subst_upper := fv_exp_subst_exp_wrt_exp_upper;
+  *)
+
+  }.
+
+
+Hint Rewrite @subst_open
+  using solve [auto; try typeclasses eauto] : syntax.
+
+Hint Rewrite @subst_close
+  using solve [auto; try typeclasses eauto] : syntax.
+
+Hint Rewrite @open_close
+  using solve [auto; try typeclasses eauto] : syntax.
+
+Hint Rewrite @size_open_var
+  using solve [auto; try typeclasses eauto] : syntax.
+
+#[export] Hint Resolve subst_lc : lc.
+
+(***********************************************************************)
+(** * Rewriting / tactics *)
+(***********************************************************************)
+
+
+Ltac simp_syntax := repeat first [ 
+                       autorewrite with subst
+                     || autorewrite with open
+                     || autorewrite with close
+                     || autorewrite with fv
+                     || autorewrite with size
+                     || autorewrite with syntax
+                     ].
+
+Ltac simp_syntax_in H := repeat first [ 
+                       autorewrite with subst in H
+                     || autorewrite with open in H
+                     || autorewrite with close in H
+                     || autorewrite with fv in H 
+                     || autorewrite with size in H
+                     || autorewrite with syntax in H
+                     ].
+
+
+Lemma lc_body
+     : forall {A1 A2:Set} {a1 : A1}{a2 : A2}{v} `{SubstTheory A1 A2 v}, 
+    (forall x, lc (open a1 (v x))) -> lc a2 -> lc (open a1 a2).
+Proof.
+  intros.
+  pick fresh x for (fv a1). 
+  rewrite (subst_intro x); auto.
+  apply subst_lc; eauto.
+Qed.
+
+#[export] Hint Resolve lc_body : lc.
+
+
+(***********************************************************************)
+(** * Notations *)
+(***********************************************************************)
+
+(** Many common applications of opening replace index zero with an
+    expression or variable.  The following definition provides a
+    convenient shorthand for such uses.  Note that the order of
+    arguments is switched relative to the definition above.  For
+    example, [e ^ x] can be read as "substitute the variable [x]
+    for index [0] in [e]".
+*)
+
+Declare Scope syntax_scope.
+Module SyntaxNotations.
+Notation "[ z ~> u ] e" := (subst u z e) (at level 0) : syntax_scope.
+Notation "e ^ x"        := (open x e) : syntax_scope.
+End SyntaxNotations.
+
