DDC/src/subst.v
@@ -1,3 +1,4 @@
+Require Export ssreflect.
 Require Export Qual.metalib.
 Require Export Qual.tactics.
 Require Export Qual.labels. 
@@ -7,43 +8,44 @@ Require Export Qual.uniq.
 Set Implicit Arguments.
 Open Scope grade_scope.
 
+#[local] Opaque Syntax_tm.
+#[local] Opaque Subst_tm.
+
 
 (* ----- Step ----- *)
 
-Lemma Step_substitution : forall b1 b2 a x, Step b1 b2 -> lc_tm a -> Step (subst_tm_tm a x b1) (subst_tm_tm a x b2).
+Lemma Step_substitution : forall b1 b2 a x, Step b1 b2 -> lc a -> Step (subst a x b1) (subst a x b2).
 Proof.
   intros. induction H.
-  all: try solve [simpl; econstructor; eauto using subst_tm_tm_lc_tm]. 
-  - simpl.
-    rewrite subst_tm_tm_open_tm_wrt_tm; auto.
-     econstructor; eauto using subst_tm_tm_lc_tm.
-     match goal with [H : lc_tm (a_Abs _ _ _) |- _ ] => inversion H end. subst.
-     pick fresh y.
-     eapply (lc_a_Abs_exists y); eauto using subst_tm_tm_lc_tm.
-     replace (a_Var_f y) with (subst_tm_tm a x (a_Var_f y)).
-     rewrite <- subst_tm_tm_open_tm_wrt_tm; auto.
-     eapply subst_tm_tm_lc_tm; eauto.
-     rewrite subst_tm_tm_var_neq; auto.
-  - simpl.
-    econstructor; eauto using subst_tm_tm_lc_tm.
+  all: try solve [simpl; econstructor; eauto using subst_lc with syntax]. 
+  - simp_syntax. 
+    (* why does simpl unfold the type class here. How to prevent that? *)
+    rewrite subst_open; auto.
+    econstructor; eauto using subst_lc.
+    pose proof (K := subst_lc (a_Abs psi A a0) a x).
+    eauto.
+    (* why does move not work here? *)
+Admitted.
+(*  - simp_syntax.
+    econstructor; eauto using subst_lc.
     inversion H. subst.
      pick fresh y.
-     eapply (lc_a_LetPair_exists y); eauto using subst_tm_tm_lc_tm.
-     replace (a_Var_f y) with (subst_tm_tm a x (a_Var_f y)).
-     rewrite <- subst_tm_tm_open_tm_wrt_tm; auto.
-     eapply subst_tm_tm_lc_tm; eauto.
-     rewrite subst_tm_tm_var_neq; auto.
-  - simpl.
-    rewrite subst_tm_tm_open_tm_wrt_tm; auto.
-    econstructor; eauto using subst_tm_tm_lc_tm.
+     eapply (lc_a_LetPair_exists y); eauto using subst_lc.
+     replace (a_Var_f y) with (subst a x (a_Var_f y)).
+     rewrite <- subst_open; auto.
+     eapply subst_lc; eauto.
+     rewrite subst_var_neq; auto.
+  - simp_syntax.
+    rewrite subst_open; auto.
+    econstructor; eauto using subst_lc.
     inversion H. subst.
      pick fresh y.
-     eapply (lc_a_LetPair_exists y); eauto using subst_tm_tm_lc_tm.
-     replace (a_Var_f y) with (subst_tm_tm a x (a_Var_f y)).
-     rewrite <- subst_tm_tm_open_tm_wrt_tm; auto.
-     eapply subst_tm_tm_lc_tm; eauto.
-     rewrite subst_tm_tm_var_neq; auto.
-Qed.
+     eapply (lc_a_LetPair_exists y); eauto using subst_lc.
+     replace (a_Var_f y) with (subst a x (a_Var_f y)).
+     rewrite <- subst_open; auto.
+     eapply subst_lc; eauto.
+     rewrite subst_var_neq; auto.
+Qed. *)
 
 
 (* --- grade --- *)
@@ -64,55 +66,52 @@ Ltac substitution_ih :=
             [(?y, ?psi0)] ++ ?P2 ++ [(?x, ?phi)] ++ ?P1 = P3 ++ [(x0, phi0)] ++ P4 -> _ |- _ ] => 
                 specialize (H3 P1 ([(y, psi0)] ++ P2) x phi  ltac:(auto) _ ltac:(eauto)); 
         simpl_env in H3;
-    rewrite subst_tm_tm_open_tm_wrt_tm in H3; eauto using CGrade_lc;
-    rewrite subst_tm_tm_var_neq in H3
+    rewrite subst_open in H3; eauto using CGrade_lc;
+    rewrite subst_var_neq in H3
     end.
 
 Lemma CGrade_Grade_substitution_CGrade : (forall P psi psi0 b,
       CGrade P psi psi0 b -> forall P1 P2 x phi, 
         P = P2 ++ [(x,phi)] ++ P1 
         -> forall a , CGrade P1 psi phi a 
-        -> CGrade (P2 ++ P1) psi psi0 (subst_tm_tm a x b)) /\
+        -> CGrade (P2 ++ P1) psi psi0 (subst a x b)) /\
       (forall P psi b, 
           Grade P psi b -> forall P1 P2 x phi, 
             P = P2 ++ [(x,phi)] ++ P1 
             -> forall a, CGrade P1 psi phi a 
-                   -> Grade (P2 ++ P1) psi (subst_tm_tm a x b)).
+                   -> Grade (P2 ++ P1) psi (subst a x b)).
 Proof.
   apply CGrade_Grade_mutual. 
   all: intros; subst.
   all: try solve [simpl; eauto].
-  all: try solve [eapply CG_Nleq; eauto  using subst_tm_tm_lc_tm, CGrade_lc] .
+  all: try solve [eapply CG_Nleq; eauto  using subst_lc, CGrade_lc] .
   all: try solve [simpl;
     fresh_apply_Grade y;
-    eauto using subst_tm_tm_lc_tm, CGrade_lc;
+    eauto using subst_lc, CGrade_lc;
     repeat spec y;
     substitution_ih;
     eauto].
   - (* Var *) 
-    destruct (x == x0).
-    + subst.
-      apply binds_mid_eq in b; auto. subst.
-      rewrite subst_tm_tm_var; auto.
-      eapply Grade_weakening; try solve_uniq.
-      match goal with [ H : CGrade _ _ _ _ |- _ ] => inversion H; clear H; subst end; auto; try done.
-    + rewrite subst_tm_tm_var_neq. auto.
-      apply binds_remove_mid in b; auto.
-      eapply G_Var; eauto.
+    substitution_var.
+    + eapply Grade_weakening; try solve_uniq.
+      invert_CGrade; subst; auto; try done.
+    + eapply G_Var; eauto.
 Qed.
 
 Lemma Grade_substitution_CGrade : forall P2 x phi P1 psi a b,
       Grade (P2 ++ x ~ phi ++ P1) psi b
     -> CGrade P1 psi phi a 
-    -> Grade (P2 ++ P1) psi (subst_tm_tm a x b).
+    -> Grade (P2 ++ P1) psi (subst a x b).
 Proof. 
   intros.
   eapply CGrade_Grade_substitution_CGrade; eauto. Qed.
 
+#[global] Hint Resolve Grade_substitution_CGrade : subst.
+
 Lemma Grade_substitution_same : forall P2 x phi P1 psi a b,
       Grade (P2 ++ x ~ phi ++ P1) psi b
     -> Grade P1 psi a 
-    -> Grade (P2 ++ P1) psi (subst_tm_tm a x b).
+    -> Grade (P2 ++ P1) psi (subst a x b).
 Proof. 
   intros.
   eapply Grade_substitution_CGrade; eauto.
@@ -121,8 +120,8 @@ Qed.
 Lemma Grade_substitution_irrel : forall P2 x phi P1 psi a b,
       Grade (P2 ++ x ~ phi ++ P1) psi b
     -> not (phi <= psi)
-    -> lc_tm a
-    -> Grade (P2 ++ P1) psi (subst_tm_tm a x b).
+    -> lc a
+    -> Grade (P2 ++ P1) psi (subst a x b).
 Proof. 
   intros.
   eapply Grade_substitution_CGrade; eauto.
@@ -131,59 +130,59 @@ Proof.
 Qed.
 
 Lemma Grade_open : forall P psi y psi0 a b,
-  y `notin` fv_tm_tm a ->
+  y `notin` fv a ->
   Grade P psi b ->
-  Grade ([(y, psi0)] ++ P) psi (open_tm_wrt_tm a (a_Var_f y)) -> 
-  Grade P psi (open_tm_wrt_tm a b).
+  Grade ([(y, psi0)] ++ P) psi (open a (a_Var_f y)) -> 
+  Grade P psi (open a b).
 Proof.
   intros.
   move: (Grade_substitution_same nil _ _ H1 H0) => ss.
-  rewrite subst_tm_tm_open_tm_wrt_tm in ss.
+  rewrite subst_open in ss.
   eauto using Grade_lc.
-  rewrite subst_tm_tm_var in ss.
-  rewrite subst_tm_tm_fresh_eq in ss; auto.
+  rewrite subst_var in ss.
+  rewrite subst_fresh_eq in ss; auto.
 Qed.
 
 Lemma Grade_open_irrel : forall P psi y psi0 a b,
-  y `notin` fv_tm_tm a ->
+  y `notin` fv a ->
   not (psi0 <= psi) ->
-  lc_tm b ->
-  Grade ([(y, psi0)] ++ P) psi (open_tm_wrt_tm a (a_Var_f y)) -> 
-  Grade P psi (open_tm_wrt_tm a b).
+  lc b ->
+  Grade ([(y, psi0)] ++ P) psi (open a (a_Var_f y)) -> 
+  Grade P psi (open a b).
 Proof.
   intros.
   move: (Grade_substitution_irrel nil _ _ H2 ltac:(auto) H1) => ss.
-  rewrite subst_tm_tm_open_tm_wrt_tm in ss.
+  rewrite subst_open in ss.
   eauto using Grade_lc.
-  rewrite subst_tm_tm_var in ss.
-  rewrite subst_tm_tm_fresh_eq in ss; auto.
+  rewrite subst_var in ss.
+  rewrite subst_fresh_eq in ss; auto.
 Qed.
 
 Lemma Grade_renaming : forall y x psi0 P psi b1, 
-    x `notin` dom P \u fv_tm_tm b1 -> 
-    y `notin` dom P \u fv_tm_tm b1 \u {{x}} -> 
-    Grade ([(y, psi0)] ++ P) psi (open_tm_wrt_tm b1 (a_Var_f y)) -> 
-    Grade ([(x, psi0)] ++ P) psi (open_tm_wrt_tm b1 (a_Var_f x)).
+    x `notin` dom P \u fv b1 -> 
+    y `notin` dom P \u fv b1 \u {{x}} -> 
+    Grade ([(y, psi0)] ++ P) psi (open b1 (a_Var_f y)) -> 
+    Grade ([(x, psi0)] ++ P) psi (open b1 (a_Var_f x)).
 Proof.
   intros.
-  rewrite (subst_tm_tm_intro y b1); auto.
+  rewrite (subst_intro y b1); auto.
   move: (Grade_uniq H1) => u. 
   destruct (q_leb psi0 psi) eqn:LE.
   - eapply Grade_substitution_same with (P2 := nil) (P1 := ([(x, psi0)] ++ P)); simpl_env.
     eapply Grade_weakening_middle; eauto. 
     eapply G_Var; eauto.
     solve_uniq.
-  - eapply Grade_substitution_irrel  with (P2 := nil) (P1 := ([(x, psi0)] ++ P)); simpl_env. 2: eauto.
+  - eapply Grade_substitution_irrel  with (P2 := nil) (P1 := ([(x, psi0)] ++ P)); simpl_env. 
     eapply Grade_weakening_middle; eauto. 
     rewrite LE. done.
-    auto.
+    eauto with lc.
 Qed. 
 
 Ltac exists_apply_Grade x :=
   let y := fresh in
   fresh_apply_Grade y; eauto;
-  eapply (@Grade_renaming x); try rewrite fv_tm_tm_close_tm_wrt_tm; auto;
-  rewrite open_tm_wrt_tm_close_tm_wrt_tm; auto.
+  eapply (@Grade_renaming x); try rewrite fv_close; auto;
+  rewrite open_close; auto.
 
 (* --- geq --- *)
 
@@ -192,12 +191,12 @@ Lemma CEq_GEq_equality_substitution :
   CEq P phi phi0 b1 b2 ->  forall P1 P2 x psi, 
         P = P2 ++ [(x,psi)] ++ P1 
        -> forall a1 a2, CEq P1 phi psi a1 a2 
-       -> CEq (P2 ++ P1) phi phi0 (subst_tm_tm a1 x b1) (subst_tm_tm a2 x b2)) /\
+       -> CEq (P2 ++ P1) phi phi0 (subst a1 x b1) (subst a2 x b2)) /\
   (forall P phi b1 b2,
   GEq P phi b1 b2 -> forall P1 P2 x psi, 
         P = P2 ++ [(x,psi)] ++ P1 
        -> forall a1 a2, CEq P1 phi psi a1 a2  
-       -> GEq (P2 ++ P1) phi (subst_tm_tm a1 x b1) (subst_tm_tm a2 x b2)). 
+       -> GEq (P2 ++ P1) phi (subst a1 x b1) (subst a2 x b2)). 
 Proof. 
   eapply CEq_GEq_mutual.
   all: intros; subst; eauto.  
@@ -214,47 +213,41 @@ Proof.
     specialize (H5 P1 ([(y, psi0)] ++ P2) x psi2 ltac:(auto) _ _ ltac:(eauto 3));
     simpl_env in H5;
     simpl_env in H5;
-    repeat rewrite subst_tm_tm_open_tm_wrt_tm in H5; eauto 3 using CEq_lc1, CEq_lc2;
-    repeat rewrite subst_tm_tm_var_neq in H5; eauto
+    repeat rewrite subst_open in H5; eauto 3 using CEq_lc1, CEq_lc2;
+    repeat rewrite subst_var_neq in H5; eauto
     end] .
   - (* Var *)
-    destruct (x == x0).
-    + subst.
-      repeat rewrite subst_tm_tm_var.
-      match goal with [ H : CEq _ _ _ _ _ |- _ ] => inversion H; subst end.
-      ++ (* 
-            psi0 <= psi -- 
-          *)
-        eapply GEq_weakening; eauto.        
-      ++
-        apply binds_mid_eq in b; auto. subst.
-        done.
-        (* 
-            here we know that not (psi0 <= psi). 
-          *)
-    + repeat rewrite subst_tm_tm_var_neq; eauto.    
-
+    substitution_var. 
+    + invert_CEq; subst.      
+      eapply GEq_weakening; eauto.        
+      done.
+    + eauto.    
   - (* CEq  - nleq *)
     move: (CEq_lc1 H0) => h1.
     move: (CEq_lc2 H0) => h2.
-    eapply CEq_Nleq; eauto using subst_tm_tm_lc_tm.
+    eapply CEq_Nleq; eauto using subst_lc.
 Qed.
 
+Lemma GEq_substitution : forall P1 P2 x psi phi b1 b2,
+  GEq (P2 ++ [(x,psi)] ++ P1) phi b1 b2
+       -> forall a1 a2, CEq P1 phi psi a1 a2  
+       -> GEq (P2 ++ P1) phi (subst a1 x b1) (subst a2 x b2). 
+Proof. intros; subst. eapply CEq_GEq_equality_substitution; eauto. Qed.
 
 Lemma GEq_open: forall P psi psi0 a1 a2 a b0 x, 
-      x \notin fv_tm_tm a -> x \notin fv_tm_tm b0 ->
+      x \notin fv a -> x \notin fv b0 ->
       CEq P psi psi0 a1 a2 ->
-      GEq ([(x, psi0)] ++ P) psi (open_tm_wrt_tm a (a_Var_f x)) (open_tm_wrt_tm b0 (a_Var_f x)) ->
-      GEq P psi (open_tm_wrt_tm a a1) (open_tm_wrt_tm b0 a2).
+      GEq ([(x, psi0)] ++ P) psi (open a (a_Var_f x)) (open b0 (a_Var_f x)) ->
+      GEq P psi (open a a1) (open b0 a2).
 Proof.
       intros.
       move: (CEq_GEq_equality_substitution) => [_ h1].
       specialize (h1 _ _  _ _ H2 P nil x psi0 ltac:(eauto) _ _ H1).
-      repeat rewrite subst_tm_tm_open_tm_wrt_tm in h1; auto.
+      repeat rewrite subst_open in h1; auto.
       eapply CEq_lc1; eauto.
       eapply CEq_lc2; eauto.
-      repeat rewrite subst_tm_tm_var in h1.
-      repeat rewrite subst_tm_tm_fresh_eq in h1; auto.
+      repeat rewrite subst_var in h1.
+      repeat rewrite subst_fresh_eq in h1; auto.
 Qed.
 
 Lemma CEq_GEq_refl : 
@@ -283,7 +276,7 @@ Qed.
 Lemma GEq_substitution_same : forall P1 P2 x psi phi b1 b2 a,
   GEq (P2 ++ [(x,psi)] ++ P1) phi b1 b2 
   -> Grade P1 phi a
-  -> GEq (P2 ++ P1) phi (subst_tm_tm a x b1) (subst_tm_tm a x b2). 
+  -> GEq (P2 ++ P1) phi (subst a x b1) (subst a x b2). 
 Proof.
   intros.
   move: CEq_GEq_equality_substitution => [_ h].
@@ -294,9 +287,9 @@ Qed.
 Lemma GEq_substitution_irrel : forall P1 P2 x psi phi b1 b2 a1 a2,
   GEq (P2 ++ [(x,psi)] ++ P1) phi b1 b2 
   -> not (psi <= phi)
-  -> lc_tm a1
-  -> lc_tm a2
-  -> GEq (P2 ++ P1) phi (subst_tm_tm a1 x b1) (subst_tm_tm a2 x b2). 
+  -> lc a1
+  -> lc a2
+  -> GEq (P2 ++ P1) phi (subst a1 x b1) (subst a2 x b2). 
 Proof.
   intros.
   move: CEq_GEq_equality_substitution => [_ h].
@@ -306,30 +299,31 @@ Proof.
 Qed.
 
 Lemma GEq_renaming : forall y x psi0 P psi b1 b2, 
-    x `notin` dom P \u fv_tm_tm b1 \u fv_tm_tm b2 -> 
-    y `notin` dom P \u fv_tm_tm b1 \u fv_tm_tm b2 \u {{x}} -> 
-    GEq ([(y, psi0)] ++ P) psi (open_tm_wrt_tm b1 (a_Var_f y)) (open_tm_wrt_tm b2 (a_Var_f y)) -> 
-    GEq ([(x, psi0)] ++ P) psi (open_tm_wrt_tm b1 (a_Var_f x)) (open_tm_wrt_tm b2 (a_Var_f x)).
+    x `notin` dom P \u fv b1 \u fv b2 -> 
+    y `notin` dom P \u fv b1 \u fv b2 \u {{x}} -> 
+    GEq ([(y, psi0)] ++ P) psi (open b1 (a_Var_f y)) (open b2 (a_Var_f y)) -> 
+    GEq ([(x, psi0)] ++ P) psi (open b1 (a_Var_f x)) (open b2 (a_Var_f x)).
 Proof.
   intros.
-  rewrite (subst_tm_tm_intro y b1); auto.
-  rewrite (subst_tm_tm_intro y b2); auto.
+  rewrite (subst_intro y b1); auto.
+  rewrite (subst_intro y b2); auto.
   move: (GEq_uniq H1) => u. 
+  eapply GEq_substitution with (P2 := nil) (P1 := ([(x, psi0)] ++ P)); simpl_env.
+  eapply GEq_weakening_middle; eauto. 
   destruct (q_leb psi0 psi) eqn:LE.
-  - eapply GEq_substitution_same with (P2 := nil) (P1 := ([(x, psi0)] ++ P)); simpl_env.
-    eapply GEq_weakening_middle; eauto. 
+  - eapply CEq_refl.
     eapply G_Var; eauto.
     solve_uniq.
-  - eapply GEq_substitution_irrel  with (P2 := nil) (P1 := ([(x, psi0)] ++ P)); auto; simpl_env. 
-    eapply GEq_weakening_middle; eauto. 
-    rewrite LE. done.
+  - eapply CEq_Nleq; eauto with lc. 
+    rewrite LE. done. 
+    solve_uniq.
 Qed. 
 
 Ltac exists_apply_GEq x :=
   let y := fresh in
   fresh_apply_GEq y; eauto;
-  eapply (@GEq_renaming x); try rewrite fv_tm_tm_close_tm_wrt_tm; auto;
-  rewrite open_tm_wrt_tm_close_tm_wrt_tm; auto.
+  eapply (@GEq_renaming x); try rewrite fv_close; auto;
+  rewrite open_close; auto.
 
 
 (* --- defeq ---- *)
@@ -341,28 +335,30 @@ Local Ltac defeq_subst_ih :=  match goal with
           |- _ ] => 
     specialize (H5 P1 ([(y, psi0)] ++ P2) x psi2 ltac:(auto) _ ltac:(eauto 3));
     simpl_env in H5;
-    repeat rewrite subst_tm_tm_open_tm_wrt_tm in H5; eauto 3 using CGrade_lc;
-    repeat rewrite subst_tm_tm_var_neq in H5; eauto end.
+    repeat rewrite subst_open in H5; eauto 3 using CGrade_lc;
+    repeat rewrite subst_var_neq in H5; eauto end.
+
+
 
 Lemma CDefEq_DefEq_substitution_CGrade : 
   (forall P phi phi0 b1 b2, CDefEq P phi phi0 b1 b2 -> forall P1 P2 x psi, 
         P = P2 ++ [(x,psi)] ++ P1 
        -> forall a, CGrade P1 phi psi a
-       -> CDefEq (P2 ++ P1) phi phi0 (subst_tm_tm a x b1) (subst_tm_tm a x b2)) /\
+       -> CDefEq (P2 ++ P1) phi phi0 (subst a x b1) (subst a x b2)) /\
   (forall P phi b1 b2, DefEq P phi b1 b2 -> forall P1 P2 x psi, 
         P = P2 ++ [(x,psi)] ++ P1 
        -> forall a, CGrade P1 phi psi a
-       -> DefEq (P2 ++ P1) phi (subst_tm_tm a x b1) (subst_tm_tm a x b2)). 
+       -> DefEq (P2 ++ P1) phi (subst a x b1) (subst a x b2)). 
 Proof. 
   apply CDefEq_DefEq_mutual.
   all: intros; subst.  
   all: try solve [eapply Eq_Refl; eauto using Grade_substitution_CGrade].
   all: try solve [eapply Eq_Beta; eauto using Grade_substitution_CGrade, Step_substitution, CGrade_lc].
-  all: try solve [simpl; eapply Eq_App; eauto using Grade_substitution_CGrade, subst_tm_tm_lc_tm, CGrade_lc].
-  all: try solve [simpl; eapply Eq_WPair; eauto using Grade_substitution_CGrade, subst_tm_tm_lc_tm, CGrade_lc].
-  all: try solve [simpl; eapply Eq_SPair; eauto using Grade_substitution_CGrade, subst_tm_tm_lc_tm, CGrade_lc].
+  all: try solve [simpl; eapply Eq_App; eauto using Grade_substitution_CGrade, subst_lc, CGrade_lc].
+  all: try solve [simpl; eapply Eq_WPair; eauto using Grade_substitution_CGrade, subst_lc, CGrade_lc].
+  all: try solve [simpl; eapply Eq_SPair; eauto using Grade_substitution_CGrade, subst_lc, CGrade_lc].
   all: try solve [repeat invert_Grade; subst;
-    simpl; fresh_apply_DefEq y; eauto 3 using subst_tm_tm_lc_tm, CGrade_lc;
+    simpl; fresh_apply_DefEq y; eauto 3 using subst_lc, CGrade_lc;
     repeat spec y;
     defeq_subst_ih] .
   all: try solve [simpl; eauto 3].
@@ -371,19 +367,20 @@ Proof.
   - eapply Eq_PiFst; eauto 1. 
     specialize (H _ _ _ _ ltac:(eauto) _ ltac:(eauto));
     simpl in H; eauto.
-  - repeat rewrite subst_tm_tm_open_tm_wrt_tm; eauto 2 using CGrade_lc.
+  - repeat rewrite subst_open; eauto 2 using CGrade_lc.
     match goal with [H2 : CGrade _ _ _ _|- _ ] => 
     specialize (H0 _ _ _ _ ltac:(eauto) _ H2);
-    specialize (H _ _ _ _ ltac:(eauto) _ H2) end. simpl in H0.
-    eapply Eq_PiSnd; eauto 3 using Grade_substitution_CGrade, subst_tm_tm_lc_tm, CGrade_lc.    
-  - repeat rewrite subst_tm_tm_open_tm_wrt_tm; eauto 2 using CGrade_lc.
+    specialize (H _ _ _ _ ltac:(eauto) _ H2) end. 
+    autorewrite with subst in H.
+    eapply Eq_PiSnd; eauto 3 using Grade_substitution_CGrade, subst_lc, CGrade_lc.    
+  - repeat rewrite subst_open; eauto 2 using CGrade_lc.
     specialize (H _ _ _ _ ltac:(eauto) _ H1); simpl in H; eauto.
-  - repeat rewrite subst_tm_tm_open_tm_wrt_tm; eauto 2 using CGrade_lc.
+  - repeat rewrite subst_open; eauto 2 using CGrade_lc.
     specialize (H _ _ _ _ ltac:(eauto) _ H1); simpl in H.
     eapply Eq_WSigmaSnd; eauto using Grade_substitution_CGrade.
   - specialize (H _ _ _ _ ltac:(eauto) _ H1); simpl in H.
     eapply Eq_SSigmaFst; eauto using Grade_substitution_CGrade.
-  - repeat rewrite subst_tm_tm_open_tm_wrt_tm; eauto 2 using CGrade_lc.
+  - repeat rewrite subst_open; eauto 2 using CGrade_lc.
     specialize (H _ _ _ _ ltac:(eauto) _ H2); simpl in H.
     eapply Eq_SSigmaSnd; eauto using Grade_substitution_CGrade.
   - eapply Eq_SumFst; eauto 1.  
@@ -394,27 +391,25 @@ Proof.
     simpl in H; eauto.
   - simpl.
     eapply Eq_Case; eauto.
-  - repeat invert_Grade; subst;
-    simpl.
-    repeat rewrite subst_tm_tm_open_tm_wrt_tm; eauto 2 using CGrade_lc.
+  - repeat rewrite subst_open; eauto 2 using CGrade_lc.
     pick fresh y and apply Eq_SubstIrrel; eauto 2. 
-    eauto using subst_tm_tm_lc_tm, CGrade_lc.    
-    eauto using subst_tm_tm_lc_tm, CGrade_lc.    
+    eauto using subst_lc, CGrade_lc.    
+    eauto using subst_lc, CGrade_lc.    
     repeat spec y.
     specialize (H2 P1 ([(y, psi)] ++ P2) x psi0).
     simpl_env in H2. specialize (H2 ltac:(auto)).
     specialize (H2 _ ltac:(eassumption)).
-    repeat rewrite subst_tm_tm_open_tm_wrt_tm in H2; eauto 2 using CGrade_lc.
-    rewrite subst_tm_tm_var_neq in H2. auto.
+    repeat rewrite subst_open in H2; eauto 2 using CGrade_lc.
+    rewrite subst_var_neq in H2. auto.
     auto.
-  - eapply CDefEq_Nleq; eauto using subst_tm_tm_lc_tm, CGrade_lc.
+  - eapply CDefEq_Nleq; eauto using subst_lc, CGrade_lc.
 Qed.
 
 Lemma DefEq_substitution_CGrade : 
   (forall P phi b1 b2, DefEq P phi b1 b2 -> forall P1 P2 x psi, 
         P = P2 ++ [(x,psi)] ++ P1 
        -> forall a, CGrade P1 phi psi a
-       -> DefEq (P2 ++ P1) phi (subst_tm_tm a x b1) (subst_tm_tm a x b2)). 
+       -> DefEq (P2 ++ P1) phi (subst a x b1) (subst a x b2)). 
 Proof.
   intros. 
   eapply CDefEq_DefEq_substitution_CGrade; eauto.
@@ -424,7 +419,7 @@ Lemma DefEq_substitution_same :
   (forall P phi b1 b2, DefEq P phi b1 b2 -> forall P1 P2 x psi, 
         P = P2 ++ [(x,psi)] ++ P1 
        -> forall a, Grade P1 phi a
-       -> DefEq (P2 ++ P1) phi (subst_tm_tm a x b1) (subst_tm_tm a x b2)). 
+       -> DefEq (P2 ++ P1) phi (subst a x b1) (subst a x b2)). 
 Proof. 
   intros.
   eapply DefEq_substitution_CGrade; eauto.
@@ -435,7 +430,7 @@ Lemma DefEq_substitution_irrel : forall (P : econtext) (psi : grade) (b1 b2 : tm
        forall (P1 P2 : list (atom * grade)) (x : atom) (phi : grade),
        P = P2 ++ [(x, phi)] ++ P1 ->
        not (phi <= psi) ->
-       forall a : tm, lc_tm a -> DefEq (P2 ++ P1) psi (subst_tm_tm a x b1) (subst_tm_tm a x b2).
+       forall a : tm, lc a -> DefEq (P2 ++ P1) psi (subst a x b1) (subst a x b2).
 Proof. 
   intros.
   eapply DefEq_substitution_CGrade; eauto.
@@ -445,31 +440,32 @@ Qed.
 
 
 Lemma DefEq_renaming : forall y x psi0 P psi b1 b2, 
-    x `notin` dom P \u fv_tm_tm b1 \u fv_tm_tm b2 -> 
-    y `notin` dom P \u fv_tm_tm b1 \u fv_tm_tm b2 \u {{x}} -> 
-    DefEq ([(y, psi0)] ++ P) psi (open_tm_wrt_tm b1 (a_Var_f y)) (open_tm_wrt_tm b2 (a_Var_f y)) -> 
-    DefEq ([(x, psi0)] ++ P) psi (open_tm_wrt_tm b1 (a_Var_f x)) (open_tm_wrt_tm b2 (a_Var_f x)).
+    x `notin` dom P \u fv b1 \u fv b2 -> 
+    y `notin` dom P \u fv b1 \u fv b2 \u {{x}} -> 
+    DefEq ([(y, psi0)] ++ P) psi (open b1 (a_Var_f y)) (open b2 (a_Var_f y)) -> 
+    DefEq ([(x, psi0)] ++ P) psi (open b1 (a_Var_f x)) (open b2 (a_Var_f x)).
 Proof.
   intros.
-  rewrite (subst_tm_tm_intro y b1); auto.
-  rewrite (subst_tm_tm_intro y b2); auto.
+  rewrite (subst_intro y b1); auto.
+  rewrite (subst_intro y b2); auto.
   move: (DefEq_uniq H1) => u. 
   destruct (q_leb psi0 psi) eqn:LE.
   - eapply DefEq_substitution_same with (P2 := nil) (P1 := ([(x, psi0)] ++ P)); simpl_env. 2: eauto.
     eapply DefEq_weakening_middle; eauto. 
     eapply G_Var; eauto.
     solve_uniq.
-  - eapply DefEq_substitution_irrel  with (P2 := nil) (P1 := ([(x, psi0)] ++ P)); simpl_env. 2: eauto.
+  - eapply DefEq_substitution_irrel  with (P2 := nil) (P1 := ([(x, psi0)] ++ P)); simpl_env.
+    2: eauto.
     eapply DefEq_weakening_middle; eauto. 
     rewrite LE. done.
-    auto.
+    eauto with lc.
 Qed. 
 
 Ltac exists_apply_DefEq x :=
   let y := fresh in
   fresh_apply_DefEq y; eauto;
-  eapply (@DefEq_renaming x); try rewrite fv_tm_tm_close_tm_wrt_tm; auto;
-  rewrite open_tm_wrt_tm_close_tm_wrt_tm; auto.
+  eapply (@DefEq_renaming x); try rewrite fv_close; auto;
+  rewrite open_close; auto.
 
 
 (* --- par ---- *)
@@ -478,50 +474,49 @@ Ltac exists_apply_DefEq x :=
 Local Ltac par_subst2_ih :=
     match goal with 
       | [H3 : forall P3 x0 phi0 P4,
-            (?y, ?psi0) :: ?P2 ++ (?x, ?phi) :: ?P1 = P3 ++ (x0, phi0) ::  P4 -> _ |- _ ] => 
+            (?y ~ ?psi0) ++ ?P2 ++ (?x ~ ?phi) ++?P1 = P3 ++ (x0 ~ phi0) ++ P4 -> _ |- _ ] => 
     specialize (H3 ([(y, psi0)] ++ P2) x phi P1 ltac:(reflexivity) _ ltac:(eassumption));
     simpl_env in H3;
-    repeat rewrite subst_tm_tm_open_tm_wrt_tm in H3; eauto 3 using CGrade_lc, Par_lc1, Par_lc2;
-    repeat rewrite subst_tm_tm_var_neq in H3 
+    repeat rewrite subst_open in H3; eauto 3 using CGrade_lc, Par_lc1, Par_lc2;
+    repeat rewrite subst_var_neq in H3 
     end.
 
 Lemma CPar_Par_substitution_CGrade : (forall P psi psi0 a a', 
   CPar P psi psi0 a a' -> forall P2 x phi P1, P = (P2 ++ [(x, phi)] ++ P1) ->
   forall b, CGrade P1 psi phi b ->
-  CPar (P2 ++ P1) psi psi0 (subst_tm_tm b x a) (subst_tm_tm b x a')) /\ (forall P psi a a', 
+  CPar (P2 ++ P1) psi psi0 (subst b x a) (subst b x a')) /\ (forall P psi a a', 
   Par P psi a a' -> forall P2 x phi P1, P = (P2 ++ [(x, phi)] ++ P1) ->
   forall b, CGrade P1 psi phi b ->
-  Par (P2 ++ P1) psi (subst_tm_tm b x a) (subst_tm_tm b x a')).
+  Par (P2 ++ P1) psi (subst b x a) (subst b x a')).
 Proof.
   apply CPar_Par_mutual.
-  all: simpl; intros; subst.
-  all: simpl; eauto using Grade_substitution_CGrade, GEq_substitution_same, GEq_substitution_irrel.
+  all: intros; subst.
+  all: simp_syntax; eauto using Grade_substitution_CGrade, GEq_substitution_same, GEq_substitution_irrel.
   (* 9 subgoals *)
-  all: repeat rewrite subst_tm_tm_open_tm_wrt_tm; eauto using CGrade_lc.
-  all: try solve [fresh_apply_Par y; eauto; repeat spec y;
-            par_subst2_ih; eauto].
-  (* 2 subgoals *)
-  - simpl_env in *. eapply Par_Refl; eauto using Grade_substitution_CGrade.
-  - simpl_env in *. eapply CPar_Nleq; eauto using CGrade_lc, subst_tm_tm_lc_tm.
+  all: repeat rewrite subst_open; eauto using CGrade_lc.
+  all: try solve [econstructor; eauto; eapply H; eauto].
+  all: try solve [fresh_apply_Par y; eauto; repeat spec y; try (eapply H; eauto);
+                  par_subst2_ih; eauto].
+  eapply CPar_Nleq; eauto using CGrade_lc, subst_lc.
 Qed.
 
 Lemma Par_substitution_CGrade : forall P2 x phi P1 psi a a', 
   Par (P2 ++ [(x, phi)] ++ P1) psi a a' -> 
   forall b, CGrade P1 psi phi b ->
-  Par (P2 ++ P1) psi (subst_tm_tm b x a) (subst_tm_tm b x a').
+  Par (P2 ++ P1) psi (subst b x a) (subst b x a').
 Proof. intros. eapply CPar_Par_substitution_CGrade; eauto. Qed.
 
 Lemma subst2 : forall x phi P1 psi a a' b, 
   Par ([(x, phi)] ++ P1) psi a a' -> 
   Grade P1 psi b ->
-  Par P1 psi (subst_tm_tm b x a) (subst_tm_tm b x a').
+  Par P1 psi (subst b x a) (subst b x a').
 Proof. intros. eapply Par_substitution_CGrade with (P2:=nil); eauto. Qed.
 
 Lemma subst2_irrel : forall x phi P1 psi a a', 
   Par ([(x, phi)] ++ P1) psi a a' -> 
   forall b, not (phi <= psi) ->
-  lc_tm b ->
-  Par P1 psi (subst_tm_tm b x a) (subst_tm_tm b x a').
+  lc b ->
+  Par P1 psi (subst b x a) (subst b x a').
 Proof.
   intros.
   eapply Par_substitution_CGrade with (P2:=nil); eauto. 
@@ -530,21 +525,21 @@ Proof.
 Qed.
 
 Lemma Par_renaming : forall y x psi0 P psi b1 b2, 
-    x `notin` dom P \u fv_tm_tm b1 \u fv_tm_tm b2 -> 
-    y `notin` dom P \u fv_tm_tm b1 \u fv_tm_tm b2 \u {{x}} -> 
-    Par ([(y, psi0)] ++ P) psi (open_tm_wrt_tm b1 (a_Var_f y)) (open_tm_wrt_tm b2 (a_Var_f y)) -> 
-    Par ([(x, psi0)] ++ P) psi (open_tm_wrt_tm b1 (a_Var_f x)) (open_tm_wrt_tm b2 (a_Var_f x)).
+    x `notin` dom P \u fv b1 \u fv b2 -> 
+    y `notin` dom P \u fv b1 \u fv b2 \u {{x}} -> 
+    Par ([(y, psi0)] ++ P) psi (open b1 (a_Var_f y)) (open b2 (a_Var_f y)) -> 
+    Par ([(x, psi0)] ++ P) psi (open b1 (a_Var_f x)) (open b2 (a_Var_f x)).
 Proof.
   intros.
-  rewrite (subst_tm_tm_intro y b1); auto.
-  rewrite (subst_tm_tm_intro y b2); auto.
+  rewrite (subst_intro y b1); auto.
+  rewrite (subst_intro y b2); auto.
   move: (Par_uniq H1) => u. 
   destruct (q_leb psi0 psi) eqn:LE.
   - eapply subst2; eauto.
     eapply Par_weakening_middle; eauto. 
     eapply G_Var; eauto.
     solve_uniq.
-  - eapply subst2_irrel; eauto.
+  - eapply subst2_irrel; eauto with lc.
     eapply Par_weakening_middle; eauto. 
     rewrite LE. done.
 Qed. 
@@ -552,32 +547,22 @@ Qed.
 Ltac exists_apply_Par x :=
   let y := fresh in
   fresh_apply_Par y; eauto;
-  eapply (@Par_renaming x); try rewrite fv_tm_tm_close_tm_wrt_tm; auto;
-  rewrite open_tm_wrt_tm_close_tm_wrt_tm; auto.
+  eapply (@Par_renaming x); try rewrite fv_close; auto;
+  rewrite open_close; auto.
 
 (* Par / CPar substitution *)
-
-Local Ltac subst5_ih :=
-    match goal with 
-      | [H3 : forall P3 P4 x0 phi0,
-            [(?y, ?psi0)] ++ ?P2 ++ [(?x, ?phi)] ++ ?P1 ~= P4 ++ [(x0, phi0)] ++ P3 -> _ |- _ ] => 
-    specialize (H3 P1 ([(y, psi0)] ++ P2) x phi ltac:(reflexivity) _ _ ltac:(eassumption));
-    simpl_env in H3;
-    repeat rewrite subst_tm_tm_open_tm_wrt_tm in H3; eauto 3 using Grade_lc, CPar_lc1, CPar_lc2;
-    repeat rewrite subst_tm_tm_var_neq in H3 
-    end.
 
 Lemma subst5_full :
  (forall P psi psi0 a a',
   CEq P psi psi0 a a' ->  forall P1 P2 x phi,
         P = P2 ++ [(x,phi)] ++ P1 
        -> forall b b', CPar P1 psi phi b b' 
-       -> CPar (P2 ++ P1) psi psi0 (subst_tm_tm b x a) (subst_tm_tm b' x a')) /\
+       -> CPar (P2 ++ P1) psi psi0 (subst b x a) (subst b' x a')) /\
   (forall P psi a a',
   GEq P psi a a' -> forall P1 P2 x phi, 
         P = P2 ++ [(x,phi)] ++ P1 
        -> forall b b', CPar P1 psi phi b b' 
-       -> Par (P2 ++ P1) psi (subst_tm_tm b x a) (subst_tm_tm b' x a')).
+       -> Par (P2 ++ P1) psi (subst b x a) (subst b' x a')).
 Proof.
   eapply CEq_GEq_mutual.
   all: intros; subst; simpl; eauto.  
@@ -596,85 +581,46 @@ Proof.
             [(?y, ?psi0)] ++ ?P2 ++ [(?x, ?phi)] ++ ?P1 = P4 ++ [(x0, phi0)] ++ P3 -> _ |- _ ] => 
     specialize (H3 P1 ([(y, psi0)] ++ P2) x phi ltac:(reflexivity) _ _ ltac:(eassumption));
     simpl_env in H3;
-    repeat rewrite subst_tm_tm_open_tm_wrt_tm in H3; eauto 3 using Grade_lc, CPar_lc1, CPar_lc2;
-    repeat rewrite subst_tm_tm_var_neq in H3 end; eauto 3 ].
-  eapply CPar_Nleq; eauto 3 using CPar_lc1, CPar_lc2, subst_tm_tm_lc_tm.
+    repeat rewrite subst_open in H3; eauto 3 using Grade_lc, CPar_lc1, CPar_lc2;
+    repeat rewrite subst_var_neq in H3 end; eauto 3 ].
+  eapply CPar_Nleq; eauto 3 using CPar_lc1, CPar_lc2, subst_lc.
 Qed.
 
 
 Lemma Par_subst3_full : forall P1 psi phi b b',
     CPar P1 psi phi b b' ->
     ((forall P psi1 psi0 a a', CPar P psi1 psi0 a a' -> forall P2 x, P = (P2 ++ [(x,phi)] ++ P1) -> psi = psi1 -> 
-    CPar (P2 ++ P1) psi1 psi0 (subst_tm_tm b x a) (subst_tm_tm b' x a'))) /\ 
+    CPar (P2 ++ P1) psi1 psi0 (subst b x a) (subst b' x a'))) /\ 
     (forall P psi1 a a', Par P psi1 a a' -> forall P2 x, P = (P2 ++ [(x,phi)] ++ P1) -> psi = psi1 ->
-    Par (P2 ++ P1) psi1 (subst_tm_tm b x a) (subst_tm_tm b' x a')).
+    Par (P2 ++ P1) psi1 (subst b x a) (subst b' x a')).
 Proof.
   intros.
   apply CPar_Par_mutual.
-  all: intros; subst; simpl; eauto 4.
+  all: intros; subst; simp_syntax; eauto 4.
   (* refl case *)
   move: (subst5_full) => [_ h]. 
   eapply h; eauto using GEq_refl.
 
-  all: repeat rewrite subst_tm_tm_open_tm_wrt_tm; eauto 2 using  CPar_lc1, CPar_lc2.
+  all: repeat rewrite subst_open; eauto 2 using  CPar_lc1, CPar_lc2.
   all: eauto.
-(*  all: try (eapply_ParIrrel; eauto 3 using CPar_lc1, CPar_lc2, subst_tm_tm_lc_tm).   *)
-
+  all: try solve [  econstructor; eauto; eapply H0; eauto ].
   all: try solve [
-  fresh_apply_Par y; eauto 3; repeat spec y;
+  fresh_apply_Par y; try eapply H0; eauto 3; repeat spec y;
   match goal with 
       | [H3 : forall P3 x0,
             [(?y, ?psi0)] ++ ?P2 ++ [(?x, ?phi)] ++ ?P1 = P3 ++ [(x0, ?phi0)] ++ ?P5 -> _ |- _ ] => 
     specialize (H3 ([(y, psi0)] ++ P2) x ltac:(reflexivity) ltac:(reflexivity));
     simpl_env in H3;
-    repeat rewrite subst_tm_tm_open_tm_wrt_tm in H3; eauto 3 using Grade_lc, CPar_lc1, CPar_lc2;
-    repeat rewrite subst_tm_tm_var_neq in H3 end; eauto 3].
-
+    repeat rewrite subst_open in H3; eauto 3 using Grade_lc, CPar_lc1, CPar_lc2;
+    repeat rewrite subst_var_neq in H3 end; eauto 3].
   destruct_uniq.
- eapply CPar_Nleq; eauto 3 using CPar_lc1, CPar_lc2, subst_tm_tm_lc_tm.
+  eapply CPar_Nleq; eauto 3 using CPar_lc1, CPar_lc2, subst_lc.
 Qed.
-
-(*
-Lemma Par_subst3_full : forall P2 phi P1 b psi b' x,
-    CPar P1 psi phi b b' ->
-    forall a a', Par (P2 ++ [(x,phi)] ++ P1) psi a a' ->
-    Par (P2 ++ P1) psi (subst_tm_tm b x a) (subst_tm_tm b' x a').
-Proof.
-  intros.
-  dependent induction H0; simpl; eauto 4.
-
-
-  (* refl case *)
-  move: (subst5_full) => [_ h]. 
-  eapply h; eauto using GEq_refl.
-
-  all: repeat rewrite subst_tm_tm_open_tm_wrt_tm; eauto 2 using  CPar_lc1, CPar_lc2.
-  all: eauto.
-  all: try (eapply_ParIrrel; eauto 3 using CPar_lc1, CPar_lc2, subst_tm_tm_lc_tm).  
-
-  all: try solve [
-  fresh_apply_Par y; eauto 3; repeat spec y;
-  match goal with 
-      | [H3 : forall P3 phi0 P4 x0,
-            CPar P4 ?psi ?phi0 ?b ?b' ->
-            [(?y, ?psi0)] ++ ?P2 ++ [(?x, ?phi)] ++ ?P1 ~= P3 ++ [(x0, phi0)] ++ P4 -> _ |- _ ] => 
-    specialize (H3  ([(y, psi0)] ++ P2) phi P1 x ltac:(eassumption) ltac:(reflexivity));
-    simpl_env in H3;
-    repeat rewrite subst_tm_tm_open_tm_wrt_tm in H3; eauto 3 using Grade_lc, CPar_lc1, CPar_lc2;
-    repeat rewrite subst_tm_tm_var_neq in H3 end; eauto 3].
-
-  eapply Par_Proj1Beta; eauto.
-  eapply IHPar; eauto.
-
-  eapply Par_Proj2Beta; eauto.
-  eapply IHPar; eauto.
-Qed.
-*)
 
 Lemma Par_subst3 : forall P1 phi b psi b' x,
     CPar P1 psi phi b b' ->
     forall a a', Par ([(x,phi)] ++ P1) psi a a' ->
-    Par P1 psi (subst_tm_tm b x a) (subst_tm_tm b' x a').
+    Par P1 psi (subst b x a) (subst b' x a').
 Proof.
   intros.
   eapply Par_subst3_full with (P2 := nil); eauto.
