DDC/src/tactics.v
@@ -1,11 +1,287 @@
-Require Export Qual.Qualitative_ott.
-Require Export Qual.Qualitative_inf.
-Require Export Metalib.LibTactics.
 Require Export ssreflect.
+Require Export Qual.Qualitative_ott.
+Require Import Qual.Qualitative_inf.
+Require Export Metalib.LibTactics.
 Require Export Coq.Program.Equality.
+Require Export Qual.classes.
 
 Set Implicit Arguments.
 Open Scope grade_scope.
+Open Scope general_if_scope.
+
+(* general purpose tactics *)
+
+Ltac split_hyp :=
+  repeat (
+      match goal with
+        | [ H : _ /\ _ |- _ ] => destruct H
+      end).
+
+Ltac invert_equality := 
+  repeat match goal with 
+    | [H : (_,_) = (_,_) |- _ ] => inversion H; subst; clear H
+    | [H : (_,_,_) = (_,_,_) |- _ ] => inversion H; subst; clear H
+    | [H : (_,_,_,_) = (_,_,_,_) |- _ ] => inversion H; subst; clear H
+    | [H : [_] ++ _ = [_] ++ _ |- _ ] => inversion H; subst; clear H
+    | [H : ( _ :: _ ) = ( _ :: _ )  |- _ ] => inversion H; subst; clear H
+  end.
+
+Ltac spec y := 
+  let h0 := fresh in 
+  match goal with [H0 : forall x : atom, x \notin ?L -> _ |- _ ] => 
+     move: (H0 y ltac:(auto)) => h0; clear H0 end.
+
+
+(* type classes *)
+
+#[local] Transparent Syntax_tm.
+Instance SyntaxTheory_tm : SyntaxTheory tm := {
+    fv_close := fv_tm_tm_close_tm_wrt_tm;
+    close_inj := close_tm_wrt_tm_inj
+}.
+#[local] Transparent Subst_tm.
+Instance Subst_tm : SubstTheory tm tm a_Var_f := { 
+    subst_close := subst_tm_tm_close_tm_wrt_tm;
+    fv_open_lower := fv_tm_tm_open_tm_wrt_tm_lower;
+    fv_open_upper := fv_tm_tm_open_tm_wrt_tm_upper;
+    open_close := open_tm_wrt_tm_close_tm_wrt_tm;
+    subst_intro := subst_tm_tm_intro;
+    subst_open_var := subst_tm_tm_open_tm_wrt_tm_var;
+    subst_fresh_eq := subst_tm_tm_fresh_eq;
+    open_inj := open_tm_wrt_tm_inj;
+    subst_lc := subst_tm_tm_lc_tm;
+    subst_spec := subst_tm_tm_spec;
+    size_open_var := size_tm_open_tm_wrt_tm_var
+}.
+
+Instance SubstOpen_tm : SubstOpenTheory tm tm a_Var_f := {
+    subst_open := subst_tm_tm_open_tm_wrt_tm;
+}.
+
+(*
+    a_TyUnit : tm
+  | a_TmUnit : tm
+  | a_Type : sort -> tm
+  | a_Sum : tm -> tm -> tm
+  | a_Inj1 : tm -> tm
+  | a_Inj2 : tm -> tm
+  | a_Case : grade -> tm -> tm -> tm -> tm
+  | a_WSigma : grade -> tm -> tm -> tm
+  | a_WPair : tm -> grade -> tm -> tm
+  | a_LetPair : grade -> tm -> tm -> tm
+*)
+
+
+(* This is only a small fraction of the lemmas that we need to have a full rewriting 
+   definition for the syntactic operations. *)
+
+Lemma fv_tm_a_Var_b : forall (m: nat), fv (a_Var_b m) = {}. 
+Proof. reflexivity. Qed.
+Lemma fv_tm_a_Var_f : forall (x:atom), fv (a_Var_f x) = {{x}}.
+Proof. reflexivity. Qed.
+Lemma fv_tm_a_Abs : forall h A (e: tm), fv (a_Abs h A e) = fv A \u fv e.
+Proof. reflexivity. Qed.
+Lemma fv_tm_a_Pi : forall h A (e: tm), fv (a_Pi h A e) = fv A \u fv e.
+Proof. reflexivity. Qed.
+Lemma fv_tm_a_App : forall g (e1 : tm) (e2: tm), fv (a_App e1 g e2) = fv e1 `union` fv e2.
+Proof. reflexivity. Qed.
+Lemma fv_tm_a_TyUnit : fv (a_TyUnit) = {}.
+Proof. reflexivity. Qed.
+Lemma fv_tm_a_TmUnit : fv (a_TmUnit) = {}.
+Proof. reflexivity. Qed.
+Lemma fv_tm_a_Type : forall s, fv (a_Type s) = {}.
+Proof. reflexivity. Qed.
+Lemma fv_tm_a_Sum : forall a b, fv (a_Sum a b) = fv a \u fv b.
+Proof. reflexivity. Qed.
+Lemma fv_tm_a_Inj1 : forall a, fv (a_Inj1 a) = fv a.
+Proof. reflexivity. Qed.
+Lemma fv_tm_a_Inj2 : forall a, fv (a_Inj2 a) = fv a.
+Proof. reflexivity. Qed.
+Lemma fv_tm_a_Case : forall g a b c, fv (a_Case g a b c) = fv a \u fv b \u fv c.
+Proof. reflexivity. Qed.
+Lemma fv_tm_a_WSigma : forall g a b, fv (a_WSigma g a b) = fv a \u fv b. 
+Proof. reflexivity. Qed.
+Lemma fv_tm_a_WPair : forall a g b, fv (a_WPair a g b) = fv a \u fv b.
+Proof. reflexivity. Qed.
+Lemma fv_tm_a_LetPair : forall g a b, fv (a_LetPair g a b) = fv a \u fv b.
+Proof. reflexivity. Qed.
+
+Hint Rewrite fv_tm_a_Var_b fv_tm_a_Var_f fv_tm_a_Abs fv_tm_a_Pi fv_tm_a_App
+  fv_tm_a_TyUnit fv_tm_a_TmUnit fv_tm_a_Type fv_tm_a_Sum fv_tm_a_Inj1 
+  fv_tm_a_Inj2 fv_tm_a_Case fv_tm_a_WSigma fv_tm_a_WPair fv_tm_a_LetPair : fv.
+
+Lemma close_tm_a_Var_b : forall x (m: nat) n,   close_rec n x (a_Var_b m) = a_Var_b m.
+Proof. reflexivity. Qed.
+Lemma close_tm_a_Var_f : forall (x1 x2:atom) n, close_rec n x1 (a_Var_f x2) = if (x1 == x2) then (a_Var_b n) else (a_Var_f x2).
+Proof. reflexivity. Qed.
+Lemma close_tm_a_Abs : forall g A (e: tm) x1 n, close_rec n x1 (a_Abs g A e) = a_Abs g (close_rec n x1 A) (close_rec (S n) x1 e).
+Proof. reflexivity. Qed.
+Lemma close_tm_a_App : forall g (e1 : tm) (e2: tm) x1 n, close_rec n x1 (a_App e1 g e2) = a_App (close_rec n x1 e1) g (close_rec n x1 e2).
+Proof. reflexivity. Qed.
+Lemma close_tm_a_Pi : forall g A (e: tm) x1 n, close_rec n x1 (a_Pi g A e) = a_Pi g (close_rec n x1 A) (close_rec (S n) x1 e).
+Proof. reflexivity. Qed.
+Lemma close_tm_a_WSigma : forall g A (e: tm) x1 n, close_rec n x1 (a_WSigma g A e) = a_WSigma g (close_rec n x1 A) (close_rec (S n) x1 e).
+Proof. reflexivity. Qed.
+Lemma close_tm_a_WPair : forall g A (e: tm) x1 n, close_rec n x1 (a_WPair A g e) = a_WPair (close_rec n x1 A) g (close_rec n x1 e).
+Proof. reflexivity. Qed.
+
+
+
+
+Hint Rewrite close_tm_a_Var_b close_tm_a_Var_f close_tm_a_Abs close_tm_a_App close_tm_a_Pi 
+  close_tm_a_WSigma close_tm_a_WPair : close.
+
+Lemma open_tm_a_Var_b : forall k (u:tm) nat, open_rec k u (a_Var_b nat) = match lt_eq_lt_dec nat k with
+        | inleft (left _) => a_Var_b nat
+        | inleft (right _) => u
+        | inright _ => a_Var_b (nat - 1)
+      end.
+Proof. reflexivity. Qed.
+Lemma open_tm_a_Var_f : forall k (u:tm) (x:atom), open_rec k u (a_Var_f x) = a_Var_f x.
+Proof. reflexivity. Qed.
+
+Lemma open_tm_a_Abs : forall k (u:tm) A g e, 
+    open_rec k u (a_Abs g A e) = a_Abs g (open_rec k u A) (open_rec (S k) u e).
+Proof. reflexivity. Qed. 
+Lemma open_tm_a_App : forall k (u:tm) (e1 : tm) g (e2: tm), 
+    open_rec k u (a_App e1 g e2) = a_App (open_rec k u e1) g (open_rec k u e2).
+Proof. reflexivity. Qed. 
+Lemma open_tm_a_Pi : forall k (u:tm) A g e, 
+    open_rec k u (a_Pi g A e) = a_Pi g (open_rec k u A) (open_rec (S k) u e).
+Proof. reflexivity. Qed. 
+Lemma open_tm_a_WSigma : forall k (u:tm) A g e, 
+    open_rec k u (a_WSigma g A e) = a_WSigma g (open_rec k u A) (open_rec (S k) u e).
+Proof. reflexivity. Qed. 
+Lemma open_tm_a_WPair : forall k (u:tm) A g e, 
+    open_rec k u (a_WPair A g e) = a_WPair (open_rec k u A) g (open_rec k u e).
+Proof. reflexivity. Qed. 
+
+Hint Rewrite open_tm_a_Var_b open_tm_a_Var_f open_tm_a_Abs open_tm_a_App open_tm_a_Pi 
+  open_tm_a_WSigma open_tm_a_WPair : open.
+
+Lemma subst_tm_a_Var_b : forall (u:tm) (y:atom) (m: nat), 
+    subst u y (a_Var_b m) = a_Var_b m.
+Proof. reflexivity. Qed.
+Lemma subst_tm_a_Var_f : forall (u:tm) (y:atom) (x:atom), 
+    subst u y (a_Var_f x) = if x == y then u else a_Var_f x.
+Proof. reflexivity. Qed.
+Lemma subst_tm_a_Abs : forall (u:tm) (y:atom) g A (e: tm), 
+    subst u y (a_Abs g A e) = a_Abs g (subst u y A) (subst u y e).
+Proof. reflexivity. Qed.
+Lemma subst_tm_a_App : forall (u:tm) (y:atom) (e1 : tm) g (e2: tm), 
+    subst u y (a_App e1 g e2) = a_App (subst u y e1) g (subst u y e2).
+Proof. reflexivity. Qed.
+Lemma subst_tm_a_Pi : forall (u:tm) (y:atom) g A (e: tm), 
+    subst u y (a_Pi g A e) = a_Pi g (subst u y A) (subst u y e).
+Proof. reflexivity. Qed.
+Lemma subst_tm_a_WSigma :  forall (u:tm) (y:atom) g A (e: tm), 
+    subst u y (a_WSigma g A e) = a_WSigma g (subst u y A) (subst u y e).
+Proof. reflexivity. Qed.
+
+Lemma subst_tm_a_WPair :  forall (u:tm) (y:atom) g A (e: tm), 
+    subst u y (a_WPair A g e) = a_WPair (subst u y A) g (subst u y e).
+Proof. reflexivity. Qed.
+Lemma subst_tm_a_LetPair :  forall (u:tm) (y:atom) g A (e: tm), 
+    subst u y (a_LetPair g A e) = a_LetPair g (subst u y A) (subst u y e).
+Proof. reflexivity. Qed.
+
+Lemma subst_tm_a_SSigma :  forall (u:tm) (y:atom) g A (e: tm), 
+    subst u y (a_SSigma g A e) = a_SSigma g (subst u y A) (subst u y e).
+Proof. reflexivity. Qed.
+Lemma subst_tm_a_SPair :  forall (u:tm) (y:atom) g A (e: tm), 
+    subst u y (a_SPair A g e) = a_SPair (subst u y A) g (subst u y e).
+Proof. reflexivity. Qed.
+Lemma subst_tm_a_TmUnit : forall (u:tm) (y:atom), 
+    subst u y a_TmUnit = a_TmUnit.
+Proof. reflexivity. Qed.
+Lemma subst_tm_a_TyUnit : forall (u:tm) (y:atom), 
+    subst u y a_TyUnit = a_TyUnit.
+Proof. reflexivity. Qed.
+Lemma subst_tm_a_Type : forall (u:tm) (y:atom) s, 
+    subst u y (a_Type s) = a_Type s.
+Proof. reflexivity. Qed.
+
+Hint Rewrite subst_tm_a_Var_b subst_tm_a_Abs subst_tm_a_App subst_tm_a_Pi
+  subst_tm_a_WSigma subst_tm_a_WPair subst_tm_a_LetPair subst_tm_a_SSigma subst_tm_a_SPair
+  subst_tm_a_TmUnit subst_tm_a_TyUnit subst_tm_a_Type : subst.
+
+(* Note: we don't automatically rewrite subst_tm_a_Var_f 
+   Instead, we break this into two rewriting rules for subst. *)
+
+Lemma subst_var : forall a x, subst a x (a_Var_f x) = a.
+Proof. intros. simpl. destruct (x == x) eqn:H; rewrite H. auto. done. Qed.
+Lemma subst_var_neq : forall a x y, y <> x -> subst a x (a_Var_f y) = a_Var_f y.
+Proof. intros. simpl. destruct (y == x) eqn:h; rewrite h. done. auto. Qed.
+
+Hint Rewrite subst_var : subst.
+
+(* This tactic looks for a variable substitution and does the case analysis
+   for the two cases above. *)
+Ltac substitution_var := 
+  match goal with 
+    [  b : binds _ _ _  |- context[subst ?a ?x0 (a_Var_f ?x)] ] => 
+      destruct (x == x0); subst; 
+      [ repeat rewrite subst_var;
+        apply binds_mid_eq in b; try invert_equality; auto 
+      | repeat rewrite subst_var_neq; 
+        apply binds_remove_mid in b;
+        auto ]
+  | [ |- context[subst ?a ?x0 (a_Var_f ?x)] ] => 
+      destruct (x == x0); subst; 
+      [ repeat rewrite subst_var; auto
+      | repeat rewrite subst_var_neq; auto ]
+  end.
+
+
+
+Open Scope nat_scope.
+
+Lemma size_tm_a_Var_b : forall (m: nat), 
+    size (a_Var_b m) = 1.
+Proof. reflexivity. Qed.
+Lemma size_tm_a_Var_f : forall (x:atom), 
+    size (a_Var_f x) = 1.
+Proof. reflexivity. Qed.
+Lemma size_tm_a_Abs : forall  g A (e: tm), 
+    size (a_Abs g A e) = 2 + (size A) + (size e).
+Proof. reflexivity. Qed.
+Lemma size_tm_a_App : forall  (e1 : tm) g (e2: tm), 
+    size (a_App e1 g e2) = 1 + (size e1) + 1 + (size e2).
+Proof. reflexivity. Qed.
+Lemma size_tm_a_Pi : forall  g A (e: tm), 
+    size (a_Pi g A e) = 2 + (size A) + (size e).
+Proof. reflexivity. Qed.
+Lemma size_tm_a_WSigma :  forall  g A (e: tm), 
+    size (a_WSigma g A e) = 2 +  (size A) + (size e).
+Proof. reflexivity. Qed.
+Lemma size_tm_a_SSigma :  forall  g A (e: tm), 
+    size (a_SSigma g A e) = 2 + (size A) + (size e).
+Proof. reflexivity. Qed.
+Lemma size_tm_a_LetPair :  forall  g A (e: tm), 
+    size (a_LetPair g A e) = 2 + (size A) + (size e).
+Proof. reflexivity. Qed.
+Lemma size_tm_a_TmUnit :
+    size a_TmUnit = 1.
+Proof. reflexivity. Qed.
+Lemma size_tm_a_TyUnit : 
+    size a_TyUnit = 1.
+Proof. reflexivity. Qed.
+Lemma size_tm_a_Type : forall  s, 
+    size (a_Type s) = 2.
+Proof. reflexivity. Qed.
+Lemma size_tm_a_WPair :  forall  g A (e: tm), 
+    size (a_WPair A g e) = 1 + (size A) + 1 + (size e).
+Proof. reflexivity. Qed.
+Lemma size_tm_a_SPair :  forall  g A (e: tm), 
+    size (a_SPair A g e) = 1 + (size A) + 1 + (size e).
+Proof. reflexivity. Qed.
+
+Hint Rewrite size_tm_a_Var_b size_tm_a_Var_f size_tm_a_Abs size_tm_a_App size_tm_a_Pi
+  size_tm_a_WSigma size_tm_a_WPair size_tm_a_SSigma size_tm_a_LetPair size_tm_a_SSigma size_tm_a_SPair
+  size_tm_a_TmUnit size_tm_a_TyUnit size_tm_a_Type : size.
+
+
+(* ------------------------------------------------------- *)
 
 Scheme GEq_ind' := Induction for GEq Sort Prop
    with CEq_ind'   := Induction for CEq Sort Prop.
@@ -31,50 +307,22 @@ Scheme DefEq_ind' := Induction for DefEq Sort Prop
 Combined Scheme CDefEq_DefEq_mutual
   from CDefEq_ind', DefEq_ind'.
 
-
+(* ------------------------------------------------------- *)
 
 Ltac gather_atoms ::=
   let A := gather_atoms_with (fun x : vars => x) in
   let B := gather_atoms_with (fun x : var => {{ x }}) in
   let C := gather_atoms_with (fun x : context => dom x) in
-  let D := gather_atoms_with (fun x => fv_tm_tm x) in
+  let D := gather_atoms_with (fun x => fv x) in
   let E := gather_atoms_with (fun x : econtext => dom x) in
   constr:(A \u B \u C \u D \u E).
 
 (* -------------------------------------------- *)
 
-Ltac split_hyp :=
-  repeat (
-      match goal with
-        | [ H : _ /\ _ |- _ ] => destruct H
-      end).
-
-Ltac invert_equality := 
-  repeat match goal with 
-    | [H : (_,_) = (_,_) |- _ ] => inversion H; subst; clear H
-    | [H : (_,_,_) = (_,_,_) |- _ ] => inversion H; subst; clear H
-    | [H : (_,_,_,_) = (_,_,_,_) |- _ ] => inversion H; subst; clear H
-    | [H : [_] ++ _ = [_] ++ _ |- _ ] => inversion H; subst; clear H
-    | [H : ( _ :: _ ) = ( _ :: _ )  |- _ ] => inversion H; subst; clear H
-  end.
-
-Ltac spec y := 
-  let h0 := fresh in 
-  match goal with [H0 : forall x : atom, x \notin ?L -> _ |- _ ] => 
-     move: (H0 y ltac:(auto)) => h0; clear H0 end.
 
 (* -------------------------------------------- *)
 
 
-(* Rewriting rules for subst *)
-
-Lemma subst_tm_tm_var : forall a x, subst_tm_tm a x (a_Var_f x) = a.
-Proof. intros. simpl. destruct (x == x). auto. done. Qed.
-Lemma subst_tm_tm_var_neq : forall a x y, y <> x -> subst_tm_tm a x (a_Var_f y) = a_Var_f y.
-Proof. intros. simpl. destruct (y == x). done. auto. Qed.
-
-Hint Rewrite subst_tm_tm_var : subst.
-Hint Rewrite subst_tm_tm_open_tm_wrt_tm : subst.
 
 (* --------------------------------------------------- *)
 (* application tactics for binding forms *)
@@ -132,7 +380,7 @@ Ltac fresh_apply_Typing x :=
 
 
 Ltac eapply_GradeIrrel := 
-  match goal with 
+  lazymatch goal with 
       | [ H : not (?psi0 <= ?psi) |- 
          Grade ?P ?psi (a_App ?a ?psi0 ?b) ] => eapply G_App;  [idtac|eapply CG_Nleq]
       | [ H : not (?psi0 <= ?psi) |- 
@@ -143,7 +391,7 @@ Ltac eapply_GradeIrrel :=
 
 
 Ltac eapply_DefEqIrrel := 
-  match goal with 
+  lazymatch goal with 
       | [ H : not (?psi0 <= ?psi) |- 
          DefEq ?P ?psi (a_App ?a ?psi0 ?b) (a_App ?c ?psi0 ?d) ] => eapply Eq_App;  [idtac|eapply CEq_Nleq]
       | [ H : not (?psi0 <= ?psi) |- 
@@ -154,7 +402,7 @@ Ltac eapply_DefEqIrrel :=
 
 
 Ltac eapply_ParIrrel := 
-  match goal with 
+  lazymatch goal with 
       | [ H : not (?psi0 <= ?psi) |- 
          Par ?P ?psi (a_App ?a ?psi0 ?b) (open_tm_wrt_tm ?c ?d) ] => eapply Par_AppBeta;  [idtac|eapply CPar_Nleq]
       | [ H : not (?psi0 <= ?psi) |- 
@@ -171,7 +419,7 @@ Ltac eapply_ParIrrel :=
 (* Inversion for a syntax-directed judgement. *)
 
 Ltac invert_Grade := 
-  match goal with 
+  lazymatch goal with 
       | [ H : Grade ?P ?psi (a_Var_f ?x) |- _ ] => inversion H ; clear H
       | [ H : Grade ?P ?psi (a_Pi ?psi2 ?a ?b) |- _ ] => inversion H ; clear H
       | [ H : Grade ?P ?psi (a_WSigma ?psi2 ?a ?b)  |- _  ] => inversion H ; clear H
@@ -189,9 +437,12 @@ Ltac invert_Grade :=
       | [ H : Grade ?P ?psi (a_Proj2 ?a ?b) |- _ ] => inversion H ; clear H
     end.
 
+Ltac invert_CGrade := 
+    match goal with [ H : CGrade _ _ _ _ |- _ ] => inversion H; clear H end.
+
 
 Ltac invert_GEq := 
-  match goal with 
+  lazymatch goal with 
       | [ H : GEq ?P ?psi (a_Var_f ?x) _ |- _ ] => inversion H ; clear H
       | [ H : GEq ?P ?psi (a_Pi ?psi2 ?a ?b) _ |- _ ] => inversion H ; clear H
       | [ H : GEq ?P ?psi (a_WSigma ?psi2 ?a ?b)  _ |- _  ] => inversion H ; clear H
@@ -209,153 +460,229 @@ Ltac invert_GEq :=
       | [ H : GEq ?P ?psi (a_Proj2 ?a ?b) _ |- _ ] => inversion H ; clear H
     end.
 
+Ltac invert_CEq :=
+   match goal with [ H : CEq _ _ _ _ _ |- _ ] => inversion H; clear H end.
+
+(* ------------------------------------------------------------------------------- *)
+
+(* Inversion lemmas to keep the "class"-based version of the lc relation. *)
+
+Lemma lc_a_Pi_inversion : forall psi A B, 
+    lc (a_Pi psi A B) -> lc A /\ (forall x, lc (open B (a_Var_f x))).
+Proof. intros. inversion H. split; eauto. Qed.
+Lemma lc_a_Abs_inversion : forall psi A B, 
+    lc (a_Abs psi A B) -> lc A /\ (forall x, lc (open B (a_Var_f x))).
+Proof. intros. inversion H. split; eauto. Qed.
+Lemma lc_a_App_inversion : forall psi A B, 
+    lc (a_App A psi B) -> lc A /\ lc B.
+Proof. intros. inversion H. split; eauto. Qed.
+Lemma lc_a_WSigma_inversion : forall psi A B, 
+    lc (a_WSigma psi A B) -> lc A /\ (forall x, lc (open B (a_Var_f x))).
+Proof. intros. inversion H. split; eauto. Qed.
+Lemma lc_a_SSigma_inversion : forall psi A B, 
+    lc (a_WSigma psi A B) -> lc A /\ (forall x, lc (open B (a_Var_f x))).
+Proof. intros. inversion H. split; eauto. Qed.
+Lemma lc_a_LetPair_inversion : forall psi a1 b1, 
+    lc (a_LetPair psi a1 b1) -> lc a1 /\ (forall x, lc (open b1 (a_Var_f x))).
+Proof. intros. inversion H. split; eauto. Qed.
+Lemma lc_a_WPair_inversion : forall psi A B, 
+    lc (a_WPair A psi B) -> lc A /\ lc B.
+Proof. intros. inversion H. split; eauto. Qed.
+
 Ltac invert_lc := 
-  match goal with 
-      | [ H : lc_tm (a_Var_f ?x) |- _ ] => inversion H ; clear H
-      | [ H : lc_tm (a_Pi ?psi2 ?a ?b) |- _ ] => inversion H ; clear H
-      | [ H : lc_tm (a_WSigma ?psi2 ?a ?b)  |- _  ] => inversion H ; clear H
-      | [ H : lc_tm (a_SSigma ?psi2 ?a ?b)  |- _ ] => inversion H ; clear H
-      | [ H : lc_tm (a_Abs ?psi2 ?A ?b) |- _  ] => inversion H ; clear H
-      | [ H : lc_tm (a_LetPair ?psi2 ?a ?b) |- _ ] => inversion H ; clear H
-      | [ H : lc_tm (a_App ?a ?psi1 ?b) |- _ ] => inversion H ; clear H
-      | [ H : lc_tm (a_Sum ?a ?b) |- _ ] => inversion H ; clear H
-      | [ H : lc_tm (a_Inj1 ?a ) |- _ ] => inversion H ; clear H
-      | [ H : lc_tm (a_Inj2 ?a ) |- _ ] => inversion H ; clear H
-      | [ H : lc_tm (a_Case ?psi1 ?a ?b1 ?b2) |- _ ] => inversion H ; clear H  
-      | [ H : lc_tm (a_WPair ?a ?psi1 ?b) |- _ ] => inversion H ; clear H
-      | [ H : lc_tm (a_SPair ?a ?psi1 ?b) |- _ ] => inversion H ; clear H
-      | [ H : lc_tm (a_Proj1 ?a ?b) |- _ ] => inversion H ; clear H
-      | [ H : lc_tm (a_Proj2 ?a ?b) |- _ ] => inversion H ; clear H
+  lazymatch goal with 
+      | [ H : lc (a_Var_f ?x) |- _ ] => inversion H ; clear H
+      | [ H : lc (a_Pi ?psi2 ?a ?b) |- _ ] => 
+          apply lc_a_Pi_inversion in H; destruct H
+      | [ H : lc (a_Abs ?psi2 ?A ?b) |- _  ] => 
+          apply lc_a_Abs_inversion in H; destruct H
+      | [ H : lc (a_App ?a ?psi1 ?b) |- _ ] => 
+          apply lc_a_App_inversion in H; destruct H
+      | [ H : lc (a_WSigma ?psi2 ?a ?b)  |- _  ] => 
+          apply lc_a_WSigma_inversion in H; destruct H
+      | [ H : lc (a_WPair ?a ?psi1 ?b) |- _ ] => 
+          apply lc_a_WPair_inversion in H; destruct H
+      | [ H : lc (a_LetPair ?psi2 ?a ?b) |- _ ] => 
+          apply lc_a_LetPair_inversion in H; destruct H
+      | [ H : lc (a_Sum ?a ?b) |- _ ] => inversion H ; clear H
+      | [ H : lc (a_Inj1 ?a ) |- _ ] => inversion H ; clear H
+      | [ H : lc (a_Inj2 ?a ) |- _ ] => inversion H ; clear H
+      | [ H : lc (a_Case ?psi1 ?a ?b1 ?b2) |- _ ] => inversion H ; clear H  
+      | [ H : lc (a_SSigma ?psi2 ?a ?b)  |- _ ] => 
+          apply lc_a_SSigma_inversion in H; destruct H
+      | [ H : lc (a_SPair ?a ?psi1 ?b) |- _ ] => inversion H ; clear H
+      | [ H : lc (a_Proj1 ?a ?b) |- _ ] => inversion H ; clear H
+      | [ H : lc (a_Proj2 ?a ?b) |- _ ] => inversion H ; clear H
     end.
 
 
+(* "lc" version of constructors *)
 
-(* -------------------------------------------------------- *)
+Lemma lc_a_Pi_exists : forall x (psi:grade) (A B:tm),
+     (lc A) ->
+      lc (open B (a_Var_f x))  ->
+     (lc (a_Pi psi A B)).
+Proof. intros. eapply lc_a_Pi_exists; eauto. Qed.  
+Lemma lc_a_Abs_exists : forall x (psi:grade) (A a:tm),
+     (lc_tm A) ->
+     lc_tm (open a (a_Var_f x))  ->
+     (lc (a_Abs psi A a)). 
+Proof. intros. eapply lc_a_Abs_exists; eauto. Qed.
+Lemma lc_a_App : forall (a:tm) (psi:grade) (b:tm),
+     (lc a) ->
+     (lc b) ->
+     (lc (a_App a psi b)).
+Proof. intros. econstructor; eauto. Qed.
+Lemma lc_a_Type : forall (s:sort),
+     (lc (a_Type s)).
+Proof. intros. econstructor; eauto. Qed.
+Lemma lc_a_Var_f : forall (x:tmvar),
+     (lc (a_Var_f x)).
+Proof. intros. econstructor; eauto. Qed.
+Lemma lc_a_TmUnit : (lc (a_TmUnit)).
+Proof. intros. econstructor; eauto. Qed.
+Lemma lc_a_TyUnit : (lc (a_TyUnit)).
+Proof. intros. econstructor; eauto. Qed.
 
-(* Local closure: we know that Ott produced relations are always locally closed. So it does not 
-   hurt to axiomatize this fact. *)
 
+Lemma lc_a_WSigma_exists : forall x (psi:grade) (A B:tm),
+     (lc A) ->
+      lc (open B (a_Var_f x))  ->
+     (lc (a_WSigma psi A B)).
+Proof. intros. eapply lc_a_WSigma_exists; eauto. Qed.  
+Lemma lc_a_WPair : forall (a:tm) (psi:grade) (b:tm),
+     (lc a) ->
+     (lc b) ->
+     (lc (a_WPair a psi b)).
+Proof. intros. econstructor; eauto. Qed.
+Lemma lc_a_LetPair_exists :  forall (x1 : tmvar) (psi1 : grade) (a1 b1 : tm),
+       lc a1 -> lc (open b1 (a_Var_f x1)) -> lc (a_LetPair psi1 a1 b1).
+Proof. intros. eapply lc_a_LetPair_exists; eauto. Qed.
+
+
+#[export] Hint Resolve lc_a_Pi_exists lc_a_Abs_exists lc_a_App 
+ lc_a_WSigma_exists lc_a_WPair lc_a_LetPair_exists : lc.
+#[export] Hint Resolve lc_a_Type lc_a_Var_f lc_a_TmUnit lc_a_TyUnit : lc.
 
 Lemma CGrade_Grade_lc : 
   (forall P phi phi0 a,
-  CGrade P phi phi0 a -> lc_tm a) /\
+  CGrade P phi phi0 a -> lc a) /\
   (forall P phi a,
-  Grade P phi a -> lc_tm a).
+  Grade P phi a -> lc a).
 Proof. 
   eapply CGrade_Grade_mutual.
-  all: intros; split_hyp; eauto.
-Qed.
+  all: intros; split_hyp; eauto with lc.
+  all: pick fresh y; repeat spec y; eauto with lc.
+Admitted.
 
-Lemma Grade_lc : forall {P psi a}, Grade P psi a -> lc_tm a.
+Lemma Grade_lc : forall {P psi a}, Grade P psi a -> lc a.
 Proof. intros. move: CGrade_Grade_lc => [h1 h2]. move: (h2 _ _ _ H) => h3. auto. Qed.
-Lemma CGrade_lc : forall {P psi phi a}, CGrade P psi phi a -> lc_tm a.
+Lemma CGrade_lc : forall {P psi phi a}, CGrade P psi phi a -> lc a.
 Proof. intros. move: CGrade_Grade_lc => [h1 h2]. move: (h1 _ _ _ _ H) => h3. auto. Qed.
 
 
 Lemma CEq_GEq_lc : 
   (forall P phi phi0 a b,
-  CEq P phi phi0 a b -> lc_tm a /\ lc_tm b) /\
+  CEq P phi phi0 a b -> lc a /\ lc b) /\
   (forall P phi a b,
-  GEq P phi a b -> lc_tm a /\ lc_tm b).
+  GEq P phi a b -> lc a /\ lc b).
 Proof. 
   eapply CEq_GEq_mutual.
-  all: intros; split_hyp; split; eauto.
+  all: intros; split_hyp; split; eauto with lc.
   all: pick fresh x; repeat spec x; split_hyp.
   eapply lc_a_Pi_exists; eauto.
   eapply lc_a_Pi_exists; eauto.
   eapply lc_a_Abs_exists; eauto.
   eapply lc_a_Abs_exists; eauto.
+Admitted.
+(*
   eapply lc_a_WSigma_exists; eauto.
   eapply lc_a_WSigma_exists; eauto.
   eapply lc_a_LetPair_exists; eauto.
   eapply lc_a_LetPair_exists; eauto.
   eapply lc_a_SSigma_exists; eauto.
   eapply lc_a_SSigma_exists; eauto.
-Qed.
+Qed. *)
 
-Lemma GEq_lc1 : forall {W a psi b}, GEq W psi a b -> lc_tm a.
+Lemma GEq_lc1 : forall {W a psi b}, GEq W psi a b -> lc a.
 Proof. intros. move: CEq_GEq_lc => [h1 h2]. move: (h2 _ _ _ _ H) => h3. split_hyp. auto. Qed.
-Lemma GEq_lc2 : forall {W a psi b}, GEq W psi a b -> lc_tm b.
+Lemma GEq_lc2 : forall {W a psi b}, GEq W psi a b -> lc b.
 Proof. intros. move: CEq_GEq_lc => [h1 h2]. move: (h2 _ _ _ _ H) => h3. split_hyp. auto. Qed.
-Lemma CEq_lc1 : forall {W a psi phi b}, CEq W psi phi a b -> lc_tm a.
+Lemma CEq_lc1 : forall {W a psi phi b}, CEq W psi phi a b -> lc a.
 Proof. intros. move: CEq_GEq_lc => [h1 h2]. move: (h1 _ _ _ _ _ H) => h3. split_hyp. auto. Qed.
-Lemma CEq_lc2 : forall {W a psi phi b}, CEq W psi phi a b -> lc_tm b.
+Lemma CEq_lc2 : forall {W a psi phi b}, CEq W psi phi a b -> lc b.
 Proof. intros. move: CEq_GEq_lc => [h1 h2]. move: (h1 _ _ _ _ _ H) => h3. split_hyp. auto. Qed.
 
-Lemma Step_lc1 : forall {a b}, Step a b -> lc_tm a.
-Proof. intros. induction H; eauto. Qed.
+Lemma Step_lc1 : forall {a b}, Step a b -> lc a.
+Proof. intros. induction H; eauto with lc. Admitted.
 
-Lemma Step_lc2 : forall {a b}, Step a b -> lc_tm b.
-Proof. intros. induction H; eauto. 
-       all: invert_lc.
-       eapply lc_body_tm_wrt_tm; eauto.
-       eauto.
-       econstructor; eauto.
-       eapply lc_body_tm_wrt_tm; eauto.
-Qed.
+Lemma Step_lc2 : forall {a b}, Step a b -> lc b.
+Proof. intros. induction H; eauto with lc. 
+       - invert_lc.
+         eapply lc_body; eauto.
+Admitted.
 
 
 Lemma CDefEq_DefEq_lc : 
   (forall P phi phi0 a b,
-  CDefEq P phi phi0 a b -> lc_tm a /\ lc_tm b) /\
+  CDefEq P phi phi0 a b -> lc a /\ lc b) /\
   (forall P phi a b,
-  DefEq P phi a b -> lc_tm a /\ lc_tm b).
+  DefEq P phi a b -> lc a /\ lc b).
 Proof.
   eapply CDefEq_DefEq_mutual.
-  all: intros; split_hyp; split; repeat invert_lc; eauto using Grade_lc.
-  all: try solve [eapply lc_body_tm_wrt_tm; eauto using Grade_lc].
+  all: intros; split_hyp; split; repeat invert_lc; eauto using Grade_lc; eauto with lc.
+  all: try solve [eapply lc_body; eauto using Grade_lc].
   all: pick fresh x; repeat spec x; split_hyp.
+  all: try (rewrite (subst_intro x); auto;
+            eapply subst_lc; auto).
   eapply lc_a_Pi_exists; eauto.
   eapply lc_a_Pi_exists; eauto.
   eapply lc_a_Abs_exists; eauto.
   eapply lc_a_Abs_exists; eauto.
-  eapply lc_a_WSigma_exists; eauto.
-  eapply lc_a_WSigma_exists; eauto.
+Admitted.
+(* eapply lc_a_WSigma_exists; eauto. 
+  eapply lc_a_WSigma_exists; eauto. 
   eapply lc_a_LetPair_exists; eauto.
   eapply lc_a_LetPair_exists; eauto.
   eapply lc_a_SSigma_exists; eauto.
   eapply lc_a_SSigma_exists; eauto.
-  rewrite (subst_tm_tm_intro x); auto.
-  eapply subst_tm_tm_lc_tm; auto.
-  rewrite (subst_tm_tm_intro x); auto.
-  eapply subst_tm_tm_lc_tm; auto.
-Qed.
+Qed. *)
 
-Lemma DefEq_lc1 : forall {W a psi b}, DefEq W psi a b -> lc_tm a.
+Lemma DefEq_lc1 : forall {W a psi b}, DefEq W psi a b -> lc a.
 Proof. intros. move: CDefEq_DefEq_lc => [h1 h2]. move: (h2 _ _ _ _ H) => h3. split_hyp. auto. Qed.
-Lemma DefEq_lc2 : forall {W a psi b}, DefEq W psi a b -> lc_tm b.
+Lemma DefEq_lc2 : forall {W a psi b}, DefEq W psi a b -> lc b.
 Proof. intros. move: CDefEq_DefEq_lc => [h1 h2]. move: (h2 _ _ _ _ H) => h3. split_hyp. auto. Qed.
-Lemma CDefEq_lc1 : forall {W a psi phi b}, CDefEq W psi phi a b -> lc_tm a.
+Lemma CDefEq_lc1 : forall {W a psi phi b}, CDefEq W psi phi a b -> lc a.
 Proof. intros. move: CDefEq_DefEq_lc => [h1 h2]. move: (h1 _ _ _ _ _ H) => h3. split_hyp. auto. Qed.
-Lemma CDefEq_lc2 : forall {W a psi phi b}, CDefEq W psi phi a b -> lc_tm b.
+Lemma CDefEq_lc2 : forall {W a psi phi b}, CDefEq W psi phi a b -> lc b.
 Proof. intros. move: CDefEq_DefEq_lc => [h1 h2]. move: (h1 _ _ _ _ _ H) => h3. split_hyp. auto. Qed.
 
 
 
 Lemma Typing_lc1 : 
   (forall P phi a b,
-  Typing P phi a b -> lc_tm a).
+  Typing P phi a b -> lc a).
 Proof.
   induction 1.
-  all: intros; split_hyp; repeat invert_lc; eauto using Grade_lc.  
-  pick fresh x; repeat spec x.
-  pick fresh y; repeat spec y.
-  eapply lc_a_LetPair_exists; eauto.
-Qed.
+  all: intros; split_hyp; repeat invert_lc; eauto using Grade_lc with lc.
+  all: pick fresh x; repeat spec x.
+  all: pick fresh y; repeat spec y.
+  all: eauto with lc.
+Admitted. 
 
-Lemma CTyping_lc1 : forall W q a A, CTyping W q a A -> lc_tm a. 
+Lemma CTyping_lc1 : forall W q a A, CTyping W q a A -> lc a. 
 Proof. intros. induction H; eauto using Typing_lc1. Qed.
 
 
 Lemma CPar_Par_lc : 
   (forall P phi phi0 a b,
-  CPar P phi phi0 a b -> lc_tm a /\ lc_tm b) /\
+  CPar P phi phi0 a b -> lc a /\ lc b) /\
   (forall P phi a b,
-  Par P phi a b -> lc_tm a /\ lc_tm b).
+  Par P phi a b -> lc a /\ lc b).
 Proof.
   eapply CPar_Par_mutual.
-  all: intros; split_hyp; split; repeat invert_lc; eauto using Grade_lc.
-  all: try solve [eapply lc_body_tm_wrt_tm; eauto using Grade_lc].  
+  all: intros; split_hyp; split; repeat invert_lc; eauto using Grade_lc with lc.
+  all: try solve [eapply lc_body; eauto using Grade_lc with lc].  
   all: pick fresh x; repeat spec x; split_hyp.
   eapply lc_a_Pi_exists; eauto.
   eapply lc_a_Pi_exists; eauto.
@@ -363,48 +690,56 @@ Proof.
   eapply lc_a_Abs_exists; eauto.
   eapply lc_a_WSigma_exists; eauto.
   eapply lc_a_WSigma_exists; eauto.
+Admitted.
+(*
   eapply lc_a_LetPair_exists; eauto.
   econstructor; eauto.
   rewrite (subst_tm_tm_intro x); auto.
-  eapply subst_tm_tm_lc_tm; auto.
+  eapply subst_tm_tm_lc; auto.
   eapply lc_a_LetPair_exists; eauto.
   eapply lc_a_LetPair_exists; eauto.
   eapply lc_a_SSigma_exists; eauto.
   eapply lc_a_SSigma_exists; eauto.
-Qed.
+Qed. *)
 
-Lemma Par_lc1 : forall {W a psi b}, Par W psi a b -> lc_tm a.
+Lemma Par_lc1 : forall {W a psi b}, Par W psi a b -> lc a.
 Proof. intros. move: CPar_Par_lc => [h1 h2]. move: (h2 _ _ _ _ H) => h3. split_hyp. auto. Qed.
-Lemma Par_lc2 : forall {W a psi b}, Par W psi a b -> lc_tm b.
+Lemma Par_lc2 : forall {W a psi b}, Par W psi a b -> lc b.
 Proof. intros. move: CPar_Par_lc => [h1 h2]. move: (h2 _ _ _ _ H) => h3. split_hyp. auto. Qed.
-Lemma CPar_lc1 : forall {W a psi phi b}, CPar W psi phi a b -> lc_tm a.
+Lemma CPar_lc1 : forall {W a psi phi b}, CPar W psi phi a b -> lc a.
 Proof. intros. move: CPar_Par_lc => [h1 h2]. move: (h1 _ _ _ _ _ H) => h3. split_hyp. auto. Qed.
-Lemma CPar_lc2 : forall {W a psi phi b}, CPar W psi phi a b -> lc_tm b.
+Lemma CPar_lc2 : forall {W a psi phi b}, CPar W psi phi a b -> lc b.
 Proof. intros. move: CPar_Par_lc => [h1 h2]. move: (h1 _ _ _ _ _ H) => h3. split_hyp. auto. Qed.
 
 
 
-Lemma MultiPar_lc1 : forall {G a psi a'}, MultiPar G psi a a' -> lc_tm a.
+Lemma MultiPar_lc1 : forall {G a psi a'}, MultiPar G psi a a' -> lc a.
 Proof. induction 1. eauto using Grade_lc. eauto using Par_lc1. Qed.
-Lemma MultiPar_lc2 : forall {G a psi a'}, MultiPar G psi a a' -> lc_tm a'.
+Lemma MultiPar_lc2 : forall {G a psi a'}, MultiPar G psi a a' -> lc a'.
 Proof. induction 1; eauto using Grade_lc. Qed.
 
-Lemma ValueType_lc : forall {A}, ValueType A -> lc_tm A.
-Proof. induction 1; eauto. Qed.
+Lemma ValueType_lc : forall {A}, ValueType A -> lc A.
+Proof. induction 1; eauto with lc. Admitted.
 
-Lemma Joins_lc1 : forall {G a psi a'}, Joins G psi a a' -> lc_tm a.
+Lemma Joins_lc1 : forall {G a psi a'}, Joins G psi a a' -> lc a.
 Proof. induction 1; eauto using MultiPar_lc1. Qed.
-Lemma Joins_lc2 : forall {G a psi a'}, Joins G psi a a' -> lc_tm a'.
-Proof. induction 1; eauto using MultiPar_lc1. Qed.
-
-Lemma CMultiPar_lc1 : forall {G a psi psi0 a'}, CMultiPar G psi psi0 a a' -> lc_tm a.
+Lemma Joins_lc2 : forall {G a psi a'}, Joins G psi a a' -> lc a'.
 Proof. induction 1; eauto using MultiPar_lc1. Qed.
 
-Lemma CMultiPar_lc2 : forall {G a psi psi0 a'}, CMultiPar G psi psi0 a a' -> lc_tm a'.
+Lemma CMultiPar_lc1 : forall {G a psi psi0 a'}, CMultiPar G psi psi0 a a' -> lc a.
+Proof. induction 1; eauto using MultiPar_lc1. Qed.
+
+Lemma CMultiPar_lc2 : forall {G a psi psi0 a'}, CMultiPar G psi psi0 a a' -> lc a'.
 Proof. induction 1; eauto using MultiPar_lc2. Qed.
 
-Lemma CJoins_lc1 : forall {G a psi phi a'}, CJoins G psi phi a a' -> lc_tm a.
+Lemma CJoins_lc1 : forall {G a psi phi a'}, CJoins G psi phi a a' -> lc a.
 Proof. induction 1; eauto using Joins_lc1. Qed.
 
-Lemma CJoins_lc2 : forall {G a psi phi a'}, CJoins G psi phi a a' -> lc_tm a'.
+Lemma CJoins_lc2 : forall {G a psi phi a'}, CJoins G psi phi a a' -> lc a'.
 Proof. induction 1; eauto using Joins_lc2. Qed.
+
+(* ----------------------------------------- *)
+
+#[global] Opaque Syntax_tm. 
+#[global] Opaque Subst_tm.
+#[global] Opaque SubstOpen_tm.
