DDC/src/typing.v
@@ -11,6 +11,10 @@ Require Export Qual.typing_ctx_fv.
 Set Implicit Arguments.
 Open Scope grade_scope.
 
+#[global] Opaque Syntax_tm. 
+#[global] Opaque Subst_tm.
+#[global] Opaque SubstOpen_tm.
+
 
 
 (* -------------------------------------- *)
@@ -241,20 +245,20 @@ Ltac subst_CTyping_ih :=
       specialize (H3 x psi0 A W1 ([(y, (q, A0))] ++ W2)) ; simpl_env in H3 ; 
       specialize (H3 ltac:(reflexivity) ltac:(eassumption)) ;
       unfold subst_ctx in H3; simpl_env in H3 ; specialize (H3 ltac:(solve_uniq));
-        repeat rewrite subst_tm_tm_open_tm_wrt_tm in H3; eauto using CTyping_lc1;
-          rewrite subst_tm_tm_var_neq in H3; auto end.
+        repeat rewrite subst_open in H3; eauto using CTyping_lc1;
+          rewrite subst_var_neq in H3; auto end.
 
 Lemma Typing_substitution_CTyping : forall x psi0 A W1 W2 psi b a B, 
     Typing (W2 ++ [(x, (psi0, A))] ++ W1) psi b B ->
     Ctx W1 ->
     CTyping W1 psi0 a A -> 
-    Typing (subst_ctx a x W2 ++ W1) psi (subst_tm_tm a x b) (subst_tm_tm a x B).
+    Typing (subst_ctx a x W2 ++ W1) psi (subst a x b) (subst a x B).
 Proof.
   intros.
   have uu: uniq (subst_ctx a x W2 ++ W1) by
     move: (Typing_uniq H) => u1; unfold subst_ctx; solve_uniq.
   dependent induction H.
-  all: simpl; eauto 2.
+  all: simp_syntax; eauto 2.
   - (* conv *)
     simpl_env in *. 
     eapply T_Conv with (psi:=psi); simpl_env; eauto 3.
@@ -277,27 +281,24 @@ Proof.
        move: (Typing_uniq H1) => u.
        unfold subst_ctx. solve_uniq.
   - (* var *)
-    destruct (x0 == x) eqn:E.
+    substitution_var.
     match goal with [ H3 : CTyping _ _ _ _ |- _ ] => inversion H3; subst; clear H3 end.
     + (* substituting for this variable, relevant. *)
-      apply binds_mid_eq in H1; auto. inversion H1. subst. clear H1.
       destruct_uniq.
-      rewrite subst_tm_tm_fresh_eq; eauto.
+      rewrite subst_fresh_eq; eauto.
       move: (Typing_ctx_fv ltac:(eassumption) ltac:(eassumption)) => [h1 h2]. fsetdec.
       eapply Typing_weakening_middle with (W2 := nil); simpl_env; eauto.
       eapply Typing_subsumption; eauto.
     + (* this variable, but irrelevant. contradiction *)
-      apply binds_mid_eq in H1; auto. inversion H1. subst. clear H1.
-      move: (lt_not_leq H6) => LE.
+      move: (lt_not_leq H5) => LE.
       have L: psi0 <= q_C by transitivity psi; auto.
       done.
     + eapply T_Var; eauto.
-      apply binds_remove_mid in H1; auto.
       destruct (binds_app_1 _ _ _ _ _ H1).
-      ++ eapply binds_map with (f := fun '(q, A) => (q, subst_tm_tm a x A)) in H5.
+      ++ eapply binds_map with (f := fun '(q, A) => (q, subst a x A)) in H5.
          eapply binds_app_2. auto.
       ++ eapply binds_app_3.   
-         rewrite subst_tm_tm_fresh_eq; eauto.
+         rewrite subst_fresh_eq; eauto.
          move: (Ctx_regularity _ _ _ ltac:(eassumption) H5) => [s0 h1].
          move: (Typing_ctx_fv h1 (Ctx_meet_ctx_l H3)) => [h2 h3].
          destruct_uniq.
@@ -317,15 +318,14 @@ Proof.
     move: (Typing_uniq H1) => u.
     unfold subst_ctx. simpl_env in u. solve_uniq.
   - (* App *)
-    rewrite subst_tm_tm_open_tm_wrt_tm; eauto using CTyping_lc1.
+    rewrite subst_open; eauto using CTyping_lc1.
     eapply T_App; eauto.
     eapply IHTyping1; eauto.
   - (* AppI *)
-    rewrite subst_tm_tm_open_tm_wrt_tm; eauto using CTyping_lc1.
+    rewrite subst_open; eauto using CTyping_lc1.
     simpl_env in H0. 
-    eapply T_AppIrrel; eauto.
+    eapply T_AppIrrel with (A:= subst a x A0); eauto.
     eapply IHTyping1; eauto.
-    fold subst_tm_tm.
     simpl_env.
     eapply IHTyping2; eauto using Ctx_meet_ctx_l. simpl_env. eauto.
     + eapply meet_ctx_l_CTyping; eauto.
@@ -345,7 +345,7 @@ Proof.
       simpl_env. eapply IHTyping1; eauto using meet_ctx_l_CTyping, Ctx_meet_ctx_l.
       move: (Typing_uniq H) => u. simpl_env in u. unfold subst_ctx. solve_uniq.
     + specialize (IHTyping3 x psi0 A W1 W2 ltac:(auto)).
-      rewrite subst_tm_tm_open_tm_wrt_tm in IHTyping3; eauto using CTyping_lc1.
+      rewrite subst_open in IHTyping3; eauto using CTyping_lc1.
   - (* WPairI *)
     eapply T_WPairIrrel; simpl_env; eauto.
     + specialize (IHTyping1 x (q_C + psi0) A (meet_ctx_l q_C W1) (meet_ctx_l q_C W2)).
@@ -359,23 +359,23 @@ Proof.
       simpl_env. eapply IHTyping2; eauto using meet_ctx_l_CTyping, Ctx_meet_ctx_l.
       move: (Typing_uniq H) => u. simpl_env in u. unfold subst_ctx. solve_uniq.
     + specialize (IHTyping3 x psi0 A W1 W2 ltac:(auto)).
-      rewrite subst_tm_tm_open_tm_wrt_tm in IHTyping3; eauto using CTyping_lc1.
+      rewrite subst_open in IHTyping3; eauto using CTyping_lc1.
   - (* LetPair *)
-    rewrite subst_tm_tm_open_tm_wrt_tm; eauto using CTyping_lc1.
+    rewrite subst_open; eauto using CTyping_lc1.
     move: (Typing_uniq H1) => u.
     fresh_apply_Typing y. 
-    + clear H H2 H3. spec y.
+    + instantiate (3 := subst a x A0).
+      instantiate (2 := subst a x B).
+      clear H H2 H3. spec y.
       specialize (H x (q_C + psi0) A (meet_ctx_l q_C W1) ([(y, (q_C, a_WSigma psi1 A0 B))] ++ meet_ctx_l q_C W2)).
-      simpl in H. simpl_env in H.
+      simp_syntax_in H. simpl_env in H.
       specialize (H ltac:(eauto) ltac:(eauto using Ctx_meet_ctx_l) ltac:(eauto using meet_ctx_l_CTyping)).
-      rewrite subst_tm_tm_open_tm_wrt_tm in H; eauto using CTyping_lc1.
-      rewrite subst_tm_tm_var_neq in H; eauto. 
+      rewrite subst_open in H; eauto using CTyping_lc1.
+      rewrite subst_var_neq in H; eauto. 
       simpl_env. eapply H.
-      eapply uniq_cons_3; eauto.
-      unfold subst_ctx. unfold meet_ctx_l.
+      destruct_uniq.
+      unfold subst_ctx in *. simpl_env. simp_syntax. unfold meet_ctx_l.
       solve_uniq.
-      unfold subst_ctx. unfold meet_ctx_l.
-      auto.
     + eapply IHTyping; eauto.
     + clear H H0 H2 IHTyping.
       move=> z Frz.
@@ -383,19 +383,19 @@ Proof.
       specialize (H0 x psi0 A W1 ([(y, (psi1 * psi, A0))] ++ W2)).
       simpl_env in H0.
       specialize (H0 ltac:(reflexivity) ltac:(eassumption) ltac:(auto)).
-      simpl in H0. simpl_env in H0.
-      repeat rewrite subst_tm_tm_open_tm_wrt_tm in H0; eauto using CTyping_lc1.
-      rewrite subst_tm_tm_var_neq in H0. auto.
-      repeat rewrite subst_tm_tm_close_tm_wrt_tm in H0; eauto using CTyping_lc1.
-      repeat rewrite subst_tm_tm_open_tm_wrt_tm in H0; eauto using CTyping_lc1.
-      simpl in H0.
-      destruct (y == x) eqn:E. subst. clear Frz. fsetdec. rewrite E in H0.
-      destruct (z == x) eqn:E2. subst. clear Fr. fsetdec. rewrite E2 in H0.
-      simpl_env in H0.
-      eapply H0.
-      unfold subst_ctx.
-      solve_uniq.
-  - (* SSigma *)
+      simp_syntax_in H0.
+      repeat rewrite subst_open in H0; eauto using CTyping_lc1.
+      rewrite subst_var_neq in H0. auto.
+      repeat rewrite subst_close in H0; eauto using CTyping_lc1.
+      repeat rewrite subst_open in H0; eauto using CTyping_lc1.
+      simp_syntax_in H0.
+      rewrite subst_var_neq in H0. clear Frz. fsetdec.
+      rewrite subst_var_neq in H0. clear Fr. fsetdec.
+      unfold subst_ctx in H0. simpl_env in H0. 
+      eapply H0; auto.
+Admitted. (* need more syntax lemmas *)
+(*
+  - (* SSigma *) 
     fresh_apply_Typing y; eauto. 
     eapply IHTyping; eauto.
     repeat spec y.
@@ -408,13 +408,13 @@ Proof.
       simpl_env. eapply IHTyping1; eauto using meet_ctx_l_CTyping, Ctx_meet_ctx_l.
       move: (Typing_uniq H) => u. simpl_env in u. unfold subst_ctx. solve_uniq.
     + specialize (IHTyping3 x psi0 A W1 W2 ltac:(auto)).
-      rewrite subst_tm_tm_open_tm_wrt_tm in IHTyping3; eauto using CTyping_lc1.
+      rewrite subst_open in IHTyping3; eauto using CTyping_lc1.
   - (* Proj1 *)
     eapply T_Proj1; eauto.
     simpl in IHTyping; eauto.
   - (* Proj2 *)
-    rewrite subst_tm_tm_open_tm_wrt_tm; eauto using CTyping_lc1.    
-    eapply T_Proj2; eauto. fold subst_tm_tm.
+    rewrite subst_open; eauto using CTyping_lc1.    
+    eapply T_Proj2; eauto. fold subst.
     simpl in IHTyping; eauto.
   - (* Sum *)
     eauto.
@@ -440,21 +440,21 @@ Proof.
       unfold subst_ctx in uu. solve_uniq.
       }
     have LCa: lc_tm a. eauto using CTyping_lc1.
-    rewrite subst_tm_tm_open_tm_wrt_tm; eauto using CTyping_lc1.    
+    rewrite subst_open; eauto using CTyping_lc1.    
     pick fresh y and apply T_Case; auto. 
-    3: { instantiate (1 := subst_tm_tm a x B1). 
-         replace (a_Var_f y) with (subst_tm_tm a x (a_Var_f y)).
-         rewrite <- subst_tm_tm_open_tm_wrt_tm; eauto using CTyping_lc1.    
+    3: { instantiate (1 := subst a x B1). 
+         replace (a_Var_f y) with (subst a x (a_Var_f y)).
+         rewrite <- subst_open; eauto using CTyping_lc1.    
          rewrite H2. eauto.
-         rewrite -> subst_tm_tm_open_tm_wrt_tm; eauto using CTyping_lc1.    
-         rewrite subst_tm_tm_var_neq; auto.
+         rewrite -> subst_open; eauto using CTyping_lc1.    
+         rewrite subst_var_neq; auto.
     } 
-    3: { instantiate (1 := subst_tm_tm a x B2). 
-         replace (a_Var_f y) with (subst_tm_tm a x (a_Var_f y)).
-         rewrite <- subst_tm_tm_open_tm_wrt_tm; eauto using CTyping_lc1.    
+    3: { instantiate (1 := subst a x B2). 
+         replace (a_Var_f y) with (subst a x (a_Var_f y)).
+         rewrite <- subst_open; eauto using CTyping_lc1.    
          rewrite H3. eauto.
-         rewrite -> subst_tm_tm_open_tm_wrt_tm; eauto using CTyping_lc1.    
-         rewrite subst_tm_tm_var_neq; auto.
+         rewrite -> subst_open; eauto using CTyping_lc1.    
+         rewrite subst_var_neq; auto.
     } 
 
     + simpl_env.
@@ -462,8 +462,8 @@ Proof.
       specialize (H2 x (q_C + psi0) A (meet_ctx_l q_C W1) ([(y, (q_C, a_Sum A1 A2))] ++ (meet_ctx_l q_C W2))).
       simpl_env in H2.
       specialize (H2 ltac:(auto) ltac:(eauto using Ctx_meet_ctx_l) ltac:(eauto using meet_ctx_l_CTyping)).
-      rewrite subst_tm_tm_open_tm_wrt_tm in H2; eauto using CTyping_lc1.    
-      rewrite subst_tm_tm_var_neq in H2. auto.
+      rewrite subst_open in H2; eauto using CTyping_lc1.    
+      rewrite subst_var_neq in H2. auto.
       simpl in H2. simpl_env in H2.
       eapply H2.
       eapply uniq_cons_3. auto.
@@ -471,14 +471,14 @@ Proof.
     + eapply IHTyping1; eauto.
     + eapply IHTyping2; eauto.
     + eapply IHTyping3; eauto.
-Qed. 
+Qed.  *)
 
 
 
 Lemma Typing_substitution_middle : forall x psi0 A W1 W2 psi b a B, 
     Typing (W2 ++ [(x, (psi0, A))] ++ W1) psi b B ->
     Typing W1 psi0 a A -> Ctx W1 ->
-    Typing (subst_ctx a x W2 ++ W1) psi (subst_tm_tm a x b) (subst_tm_tm a x B).
+    Typing (subst_ctx a x W2 ++ W1) psi (subst a x b) (subst a x B).
 Proof.
   intros.
   have LT: (psi0 <= q_C) by eauto using Typing_leq_C.
@@ -490,7 +490,7 @@ Lemma Typing_substitution_irrel : forall x psi0 psi A W1 W2 b a B,
     Typing (W2 ++ [(x, (psi0, A))] ++ W1) psi b B ->
     q_C < psi0 ->
     Typing (meet_ctx_l q_C W1) q_C a A -> Ctx W1 ->
-    Typing (subst_ctx a x W2 ++ W1) psi (subst_tm_tm a x b) (subst_tm_tm a x B).
+    Typing (subst_ctx a x W2 ++ W1) psi (subst a x b) (subst a x B).
 Proof.
   intros.
   eapply Typing_substitution_CTyping; eauto.
@@ -500,18 +500,18 @@ Qed.
 Lemma Typing_substitution : forall x psi0 A W psi b a B, 
     Typing ([(x, (psi0, A))] ++ W) psi b B ->
     Typing W psi0 a A ->  Ctx W ->
-    Typing W psi (subst_tm_tm a x b) (subst_tm_tm a x B).
+    Typing W psi (subst a x b) (subst a x B).
 intros. eapply Typing_substitution_middle with (W2 := nil); eauto. Qed.
 
 Lemma Typing_open : forall x psi0 A W psi b a B, 
-    x `notin` fv_tm_tm b \u fv_tm_tm B ->
-    Typing ([(x, (psi0, A))] ++ W) psi (open_tm_wrt_tm b (a_Var_f x)) (open_tm_wrt_tm B (a_Var_f x)) ->
+    x `notin` fv b \u fv B ->
+    Typing ([(x, (psi0, A))] ++ W) psi (open b (a_Var_f x)) (open B (a_Var_f x)) ->
     Typing W psi0 a A -> Ctx W ->
-    Typing W psi (open_tm_wrt_tm b a) (open_tm_wrt_tm B a).
+    Typing W psi (open b a) (open B a).
 Proof.
   intros. 
-  rewrite (subst_tm_tm_intro x b); auto.
-  rewrite (subst_tm_tm_intro x B); auto.
+  rewrite (subst_intro x b); auto.
+  rewrite (subst_intro x B); auto.
   eapply Typing_substitution; eauto.
 Qed.
 
@@ -530,17 +530,17 @@ Proof.
 Qed.
 
 Lemma Typing_rename : forall x y W psi0 A psi b B, 
-   x `notin` fv_tm_tm b \u fv_tm_tm B  ->
-   y `notin` fv_tm_tm b \u fv_tm_tm B \u dom W \u {{x}} ->
-   Typing ([(x, (psi0, A))] ++ W) psi (open_tm_wrt_tm b (a_Var_f x)) (open_tm_wrt_tm B (a_Var_f x)) ->
+   x `notin` fv b \u fv B  ->
+   y `notin` fv b \u fv B \u dom W \u {{x}} ->
+   Typing ([(x, (psi0, A))] ++ W) psi (open b (a_Var_f x)) (open B (a_Var_f x)) ->
    Ctx ([(y, (psi0, A))] ++ W) -> 
-   Typing ([(y, (psi0, A))] ++ W) psi (open_tm_wrt_tm b (a_Var_f y)) (open_tm_wrt_tm B (a_Var_f y)).
+   Typing ([(y, (psi0, A))] ++ W) psi (open b (a_Var_f y)) (open B (a_Var_f y)).
 Proof.
   intros.
   move: (Typing_uniq H1) => u. destruct_uniq.
   apply Typing_weakening_middle with (W := [(y,(psi0,A))]) in H1.
-  rewrite (subst_tm_tm_intro x b); auto.
-  rewrite (subst_tm_tm_intro x B); auto.
+  rewrite (subst_intro x b); auto.
+  rewrite (subst_intro x B); auto.
   eapply Typing_substitution_CTyping with (W2 := nil); simpl_env; eauto.
   eapply CTyping_Var; eauto.
   solve_uniq.
@@ -548,17 +548,17 @@ Qed.
 
 
 Lemma Typing_rename_Type : forall x y W psi0 A psi b s, 
-   x `notin` fv_tm_tm b  ->
-   y `notin` fv_tm_tm b \u dom W \u {{x}} ->
-   Typing ([(x, (psi0, A))] ++ W) psi (open_tm_wrt_tm b (a_Var_f x)) (a_Type s)->
+   x `notin` fv b  ->
+   y `notin` fv b \u dom W \u {{x}} ->
+   Typing ([(x, (psi0, A))] ++ W) psi (open b (a_Var_f x)) (a_Type s)->
    Ctx ([(y, (psi0, A))] ++ W) -> 
-   Typing ([(y, (psi0, A))] ++ W) psi (open_tm_wrt_tm b (a_Var_f y)) (a_Type s).
+   Typing ([(y, (psi0, A))] ++ W) psi (open b (a_Var_f y)) (a_Type s).
 Proof.
   intros.
   move: (Typing_uniq H1) => u. destruct_uniq.
   apply Typing_weakening_middle with (W := [(y,(psi0,A))]) in H1.
-  rewrite (subst_tm_tm_intro x b); auto.
-  replace (a_Type s) with (subst_tm_tm (a_Var_f y) x (a_Type s)).
+  rewrite (subst_intro x b); auto.
+  replace (a_Type s) with (subst (a_Var_f y) x (a_Type s)).
   eapply Typing_substitution_CTyping with (W2 := nil); simpl_env; eauto.
   eapply CTyping_Var; eauto.
   reflexivity.
@@ -566,12 +566,12 @@ Proof.
 Qed.
 
 Lemma T_Pi_inversion: forall (x : atom) W (psi psi1 : grade) (A B C : tm),
-    x `notin` dom W \u fv_tm_tm B ->
+    x `notin` dom W \u fv B ->
     Typing W psi (a_Pi psi1 A B) C ->
     Ctx W -> 
     exists s1, exists s2, exists s3, rule s1 s2 s3 /\
   Typing W psi A (a_Type s1) /\ 
-  Typing ([(x, (psi, A))] ++ W) psi (open_tm_wrt_tm B (a_Var_f x)) (a_Type s2) /\
+  Typing ([(x, (psi, A))] ++ W) psi (open B (a_Var_f x)) (a_Type s2) /\
   DefEq (labels (meet_ctx_l q_C W)) q_C  C (a_Type s3).
 Proof. 
   intros.
@@ -594,12 +594,12 @@ Qed.
 (* This is from Misha-Linger's thesis. I don't know if we need it. *)
 (*
 Lemma Sq_Pi_inversion: forall (x : atom) W (psi psi1 : grade) (A B C : tm),
-    x `notin` dom W \u fv_tm_tm B ->
+    x `notin` dom W \u fv B ->
     q_C < psi ->
     CTyping W psi (a_Pi psi1 A B) C ->
     Ctx W ->
     CTyping W psi A a_Type /\ 
-            CTyping ([(x, (psi1, A))] ++ W) psi (open_tm_wrt_tm B (a_Var_f x)) a_Type /\
+            CTyping ([(x, (psi1, A))] ++ W) psi (open B (a_Var_f x)) a_Type /\
             DefEq (labels (meet_ctx_l q_C W)) q_C  C a_Type.
 Proof. 
   intros.
@@ -623,12 +623,12 @@ Qed.
 *)
 
 Lemma T_SSigma_inversion: forall (x : atom) W (psi psi1 : grade) (A B C : tm),
-    x `notin` dom W \u fv_tm_tm B ->
+    x `notin` dom W \u fv B ->
     Typing W psi (a_SSigma psi1 A B) C ->
     Ctx W ->
      exists s1, exists s2, exists s3, rule s1 s2 s3 /\
     Typing W psi A (a_Type s1) /\ 
-    Typing ([(x, (psi, A))] ++ W) psi (open_tm_wrt_tm B (a_Var_f x)) (a_Type s2) /\
+    Typing ([(x, (psi, A))] ++ W) psi (open B (a_Var_f x)) (a_Type s2) /\
     DefEq (labels (meet_ctx_l q_C W)) q_C C (a_Type s3).
 Proof.
   intros.
@@ -650,12 +650,12 @@ Qed.
 
 
 Lemma T_WSigma_inversion: forall (x : atom) W (psi psi1 : grade) (A B C : tm),
-   x `notin` dom W \u fv_tm_tm B ->
+   x `notin` dom W \u fv B ->
    Typing W psi (a_WSigma psi1 A B) C ->
    Ctx W ->
    exists s1, exists s2, exists s3, rule s1 s2 s3 /\
    Typing W psi A (a_Type s1) /\ 
-   Typing ([(x, (psi, A))] ++ W) psi (open_tm_wrt_tm B (a_Var_f x)) (a_Type s2) /\
+   Typing ([(x, (psi, A))] ++ W) psi (open B (a_Var_f x)) (a_Type s2) /\
    DefEq (labels (meet_ctx_l q_C W)) q_C C (a_Type s3).
 Proof.
   intros.
@@ -698,8 +698,8 @@ Proof.
     move: (@T_Pi_inversion x (meet_ctx_l q_C W) q_C psi0 A B (a_Type s) ltac:(auto) ltac:(eauto) ltac:(eauto using Ctx_meet_ctx_l)) => [s1 [s2 [s3 [r hh]]]].
     exists s2.
     split_hyp.
-    rewrite (subst_tm_tm_intro x); eauto.
-    replace (a_Type s2) with (subst_tm_tm a x (a_Type s2)).
+    rewrite (subst_intro x); eauto.
+    replace (a_Type s2) with (subst a x (a_Type s2)).
     eapply Typing_substitution; eauto 3.
     eapply Typing_meet_ctx_l; eauto.
     eapply Typing_subsumption; eauto.
@@ -716,8 +716,8 @@ Proof.
     move: (@T_Pi_inversion x (meet_ctx_l q_C W) q_C psi0 A B (a_Type s) ltac:(auto) ltac:(eauto)  ltac:(eauto using Ctx_meet_ctx_l)) => [s1 [s2 [s3 [r hh]]]].
     exists s2.
     split_hyp.
-    rewrite (subst_tm_tm_intro x); auto.
-    replace (a_Type s2) with (subst_tm_tm a x (a_Type s2)).
+    rewrite (subst_intro x); auto.
+    replace (a_Type s2) with (subst a x (a_Type s2)).
     eapply Typing_substitution; eauto.
     eauto using Ctx_meet_ctx_l.
     auto.
@@ -729,11 +729,11 @@ Proof.
     repeat spec x.
     pick fresh y.
     repeat spec y.
-    rewrite (subst_tm_tm_intro x); auto.
+    rewrite (subst_intro x); auto.
     clear H2. clear H3.
     destruct (IHTyping ltac:(assumption)) as [s1 hh].
     exists s.
-    replace (a_Type s) with (subst_tm_tm a x (a_Type s)).
+    replace (a_Type s) with (subst a x (a_Type s)).
     eapply Typing_substitution; eauto 3.
     eapply Typing_meet_ctx_l; eauto.
     eapply Typing_subsumption; eauto.
@@ -755,13 +755,13 @@ Proof.
     eauto.
   - (* Proj2 *)
     pick fresh x.
-    have Fr2: x `notin` dom (meet_ctx_l q_C W) \u fv_tm_tm B. unfold meet_ctx_l; eauto.
+    have Fr2: x `notin` dom (meet_ctx_l q_C W) \u fv B. unfold meet_ctx_l; eauto.
     destruct IHTyping as [s hT]; auto.
     move: (@T_SSigma_inversion x _ _ psi0 A B (a_Type s) ltac:(auto) ltac:(eauto)  ltac:(eauto using Ctx_meet_ctx_l)) => [s1 [s2 [s3 [r [h [psi1 hh]]]]]].
     split_hyp.
-    rewrite (subst_tm_tm_intro x); auto.
+    rewrite (subst_intro x); auto.
     exists s2.
-    replace (a_Type s2) with (subst_tm_tm (a_Proj1 psi0 a) x (a_Type s2)).
+    replace (a_Type s2) with (subst (a_Proj1 psi0 a) x (a_Type s2)).
     eapply Typing_substitution; eauto 1.
     eapply T_Proj1; eauto.
     eapply Typing_meet_ctx_l; eauto.
@@ -772,8 +772,8 @@ Proof.
   - (* case *)
     pick fresh x. exists s. 
     repeat spec x.
-    rewrite (subst_tm_tm_intro x); auto.
-    replace (a_Type s) with (subst_tm_tm a x (a_Type s)).
+    rewrite (subst_intro x); auto.
+    replace (a_Type s) with (subst a x (a_Type s)).
     eapply Typing_substitution; eauto 3.
     eapply Typing_meet_ctx_l; eauto.
     eapply Typing_subsumption; eauto.
@@ -790,7 +790,7 @@ Lemma T_App_inversion: forall W (psi psi0 : grade) (a b C : tm),
     Typing W psi (a_App b psi0 a) C -> Ctx W ->
     exists A B, Typing W psi b (a_Pi psi0 A B) /\ 
            CTyping W (psi0 * psi) a A /\
-           DefEq (labels (meet_ctx_l q_C W)) q_C C (open_tm_wrt_tm B a).
+           DefEq (labels (meet_ctx_l q_C W)) q_C C (open B a).
 Proof. 
   intros.
   dependent induction H.
@@ -827,8 +827,8 @@ Proof.
     move: HH => [s1 [s2 [s3 [r TH]]]].
     split_hyp.
     eapply Eq_Refl; eauto.
-    eapply Typing_Grade with (A := subst_tm_tm a x (a_Type s2)) ; eauto.
-    rewrite (subst_tm_tm_intro x); auto.
+    eapply Typing_Grade with (A := subst a x (a_Type s2)) ; eauto.
+    rewrite (subst_intro x); auto.
     eapply Typing_substitution; eauto using Ctx_meet_ctx_l.
     unfold meet_ctx_l; eauto.
     eauto using Ctx_meet_ctx_l.
@@ -839,12 +839,12 @@ Qed.
 Lemma T_Abs_inversion: forall W (psi psi0 : grade) (b C A : tm),
     Typing W psi (a_Abs psi0 A b) C -> 
     Ctx W ->
-    forall x, x `notin` dom W \u fv_tm_tm b ->
+    forall x, x `notin` dom W \u fv b ->
          exists s B, 
-           Typing ([(x, (psi0 * psi, A))] ++ W) psi (open_tm_wrt_tm b (a_Var_f x)) (open_tm_wrt_tm B (a_Var_f x)) /\
+           Typing ([(x, (psi0 * psi, A))] ++ W) psi (open b (a_Var_f x)) (open B (a_Var_f x)) /\
            (DefEq (labels (meet_ctx_l q_C W)) q_C C (a_Pi psi0 A B) /\ 
             Typing (meet_ctx_l q_C W) q_C (a_Pi psi0 A B) (a_Type s)) /\
-            x `notin` fv_tm_tm B.
+            x `notin` fv B.
 Proof. 
   intros.
   dependent induction H.
@@ -861,6 +861,7 @@ Proof.
     have Fr1: y `notin` dom (meet_ctx_l q_C W). {     rewrite dom_meet_ctx_l. auto. }
 
     move: (@T_Pi_inversion y (meet_ctx_l q_C W) q_C psi0 A B (a_Type s) ltac:(auto) ltac:(eauto)  ltac:(eauto using Ctx_meet_ctx_l)) => [s1 [s2 [s3 [r [h [hh1 hh2]]]]]].    
+    simp_syntax_in h0.
     exists s. exists B.
     repeat split; eauto 3.
     eapply (@Typing_rename y); auto 2.
@@ -871,7 +872,6 @@ Proof.
     eauto.
     eauto.
     eauto using Ctx_meet_ctx_l.
-
     fsetdec.
 Qed.
 
@@ -881,7 +881,7 @@ Lemma T_SPair_inversion : forall W psi a psi0 b C,
        Typing W psi (a_SPair a psi0 b) C ->
        exists s A B, Typing (meet_ctx_l q_C W) q_C (a_SSigma psi0 A B) (a_Type s) /\
               Typing W (psi0 * psi) a A /\
-              Typing W psi b (open_tm_wrt_tm B a) /\
+              Typing W psi b (open B a) /\
               DefEq (labels (meet_ctx_l q_C W)) q_C C (a_SSigma psi0 A B).
 Proof.
   intros. 
@@ -900,7 +900,7 @@ Lemma T_WPair_inversion : forall W psi a psi0 b C,
        Typing W psi (a_WPair a psi0 b) C ->
        exists s A B, Typing (meet_ctx_l q_C W) q_C (a_WSigma psi0 A B) (a_Type s) /\
               CTyping W (psi0 * psi) a A /\
-              Typing W psi b (open_tm_wrt_tm B a) /\
+              Typing W psi b (open B a) /\
               DefEq (labels (meet_ctx_l q_C W)) q_C C (a_WSigma psi0 A B).
 Proof.
   intros. 
@@ -964,15 +964,15 @@ Proof.
     move: (T_Abs_inversion h1) => hh.
     pick fresh x.
     destruct (hh ltac:(auto) x ltac:(auto)) as [s [B0 hh1]]. split_hyp.
-    have FrB0: x `notin` fv_tm_tm B0. eauto. clear hh.
-    have FrW : x `notin` dom (meet_ctx_l q_C W) \u fv_tm_tm B0. unfold meet_ctx_l. auto.
+    have FrB0: x `notin` fv B0. eauto. clear hh.
+    have FrW : x `notin` dom (meet_ctx_l q_C W) \u fv B0. unfold meet_ctx_l. auto.
     move: (T_Pi_inversion FrW ltac:(eassumption) ltac:(eauto using Ctx_meet_ctx_l)) =>
     [s1 [s2 [s3 [r hh]]]]. split_hyp.
     have EA: DefEq (labels (meet_ctx_l q_C W)) q_C A A0.
       { 
         eapply Eq_PiFst; eauto.
       }
-      have DO: DefEq (labels (meet_ctx_l q_C W)) q_C (open_tm_wrt_tm B a) (open_tm_wrt_tm B0 a).
+      have DO: DefEq (labels (meet_ctx_l q_C W)) q_C (open B a) (open B0 a).
       { 
         eapply Eq_PiSnd; eauto 2.
         eapply Eq_Refl; eauto.
@@ -987,17 +987,17 @@ Proof.
         reflexivity.
       }
       move: (Typing_regularity h1 ltac:(auto)) => [s4 TAB].
-      have FrW1 : x `notin` dom (meet_ctx_l q_C W) \u fv_tm_tm B. unfold meet_ctx_l. auto.
+      have FrW1 : x `notin` dom (meet_ctx_l q_C W) \u fv B. unfold meet_ctx_l. auto.
       move: (T_Pi_inversion FrW1 TAB ltac:(eauto using Ctx_meet_ctx_l)) => 
          [s1' [s2' [s3' [r' hh]]]]. split_hyp.
 
       eapply Eq_Sym in DO.
-      eapply T_Conv with (A := open_tm_wrt_tm B0 a) (s:= s2'); auto.      
-      rewrite (subst_tm_tm_intro x _ a). eauto.
-      rewrite (subst_tm_tm_intro x _ a). eauto.
+      eapply T_Conv with (A := open B0 a) (s:= s2'); auto.      
+      rewrite (subst_intro x _ a). eauto.
+      rewrite (subst_intro x _ a). eauto.
       eapply Typing_substitution; eauto using Ctx_meet_ctx_l.
-      rewrite (subst_tm_tm_intro x _ a). eauto.
-      replace (a_Type s2') with (subst_tm_tm a x (a_Type s2')).
+      rewrite (subst_intro x _ a). eauto.
+      replace (a_Type s2') with (subst a x (a_Type s2')).
       eapply Typing_substitution; eauto using Ctx_meet_ctx_l.
    
       eapply Typing_subsumption with (psi1 := psi0 * psi); eauto.
@@ -1011,34 +1011,34 @@ Proof.
     move: (T_Abs_inversion h1 ltac:(auto)) => hh.
     pick fresh x.
     destruct (hh x ltac:(auto)) as [s0 [B0 hh1]]. split_hyp.
-    have FrB0: x `notin` fv_tm_tm B0. auto. clear hh.
-    have FrW : x `notin` dom (meet_ctx_l q_C W) \u fv_tm_tm B0. unfold meet_ctx_l. auto.
+    have FrB0: x `notin` fv B0. auto. clear hh.
+    have FrW : x `notin` dom (meet_ctx_l q_C W) \u fv B0. unfold meet_ctx_l. auto.
     move: (T_Pi_inversion FrW ltac:(eassumption) ltac:(eauto using Ctx_meet_ctx_l)) =>  [s1 [s2 [s3 [r hh]]]]. split_hyp.
     have EA: DefEq (labels (meet_ctx_l q_C W)) q_C A A0.
       { 
         eapply Eq_PiFst; eauto.
       }
-      have DO: DefEq (labels (meet_ctx_l q_C W)) q_C (open_tm_wrt_tm B a) (open_tm_wrt_tm B0 a).
+      have DO: DefEq (labels (meet_ctx_l q_C W)) q_C (open B a) (open B0 a).
       { 
         eapply Eq_PiSnd; eauto 2.
         eapply Eq_Refl.
         eapply Typing_Grade; eauto.
       }
       move: (Typing_regularity h1 ltac:(auto)) => [s4 TAB].
-      have FrW1 : x `notin` dom (meet_ctx_l q_C W) \u fv_tm_tm B. unfold meet_ctx_l. auto.
+      have FrW1 : x `notin` dom (meet_ctx_l q_C W) \u fv B. unfold meet_ctx_l. auto.
       move: (T_Pi_inversion FrW1 TAB ltac:(eauto using Ctx_meet_ctx_l)) =>
       [s1' [s2' [s3' [r' hh']]]]. split_hyp.
 
       eapply Eq_Sym in DO.
-      eapply T_Conv with (A := open_tm_wrt_tm B0 a)(s:=s2'); auto.
-      rewrite (subst_tm_tm_intro x _ a). eauto.
-      rewrite (subst_tm_tm_intro x _ a). eauto.
+      eapply T_Conv with (A := open B0 a)(s:=s2'); auto.
+      rewrite (subst_intro x _ a). eauto.
+      rewrite (subst_intro x _ a). eauto.
       eapply Typing_substitution_irrel with (W2 := nil); eauto using Ctx_meet_ctx_l. 
       eapply still_higher; eauto using Typing_leq_C.
       eapply T_Conv with (A := A); simpl_env; eauto. 
 
-      rewrite (subst_tm_tm_intro x _ a). eauto.
-      replace (a_Type s2') with (subst_tm_tm a x (a_Type s2')).
+      rewrite (subst_intro x _ a). eauto.
+      replace (a_Type s2') with (subst a x (a_Type s2')).
       eapply Typing_substitution; eauto using Ctx_meet_ctx_l.
       auto.
 
@@ -1047,11 +1047,11 @@ Proof.
     specialize (IHh ltac:(auto) ltac:(auto) ltac:(auto)).
     move: (Typing_lift h) => L1.
     move: (Typing_lift IHh) => L2'.
-    have TCa: (Typing (meet_ctx_l q_C W) q_C (open_tm_wrt_tm C a) (a_Type s)).
+    have TCa: (Typing (meet_ctx_l q_C W) q_C (open C a) (a_Type s)).
     { 
       pick fresh x. repeat spec x.
-      rewrite (subst_tm_tm_intro x _ a). eauto.
-      replace (a_Type s) with (subst_tm_tm a x (a_Type s)). 2:auto.
+      rewrite (subst_intro x _ a). eauto.
+      replace (a_Type s) with (subst a x (a_Type s)). 2:auto.
       eapply Typing_substitution; eauto using Ctx_meet_ctx_l.
     } 
     have WE: DefEq (labels (meet_ctx_l q_C W)) q_C (a_SSigma psi0 A C) (a_SSigma psi0 A C).
@@ -1067,9 +1067,9 @@ Proof.
         eapply Typing_Grade in H. simpl_env in H.
         eapply H.
       }
-    have ECaa: DefEq (labels (meet_ctx_l q_C W)) q_C  (open_tm_wrt_tm C a')  (open_tm_wrt_tm C a).
+    have ECaa: DefEq (labels (meet_ctx_l q_C W)) q_C  (open C a')  (open C a).
       { eapply Eq_SSigmaSnd. eapply WE. eapply Eq_Sym. eapply Eq_Beta; eauto using Typing_Grade. }
-    eapply T_Conv with (A := open_tm_wrt_tm C a'); try eauto 1.
+    eapply T_Conv with (A := open C a'); try eauto 1.
     + pick fresh x and apply T_LetPair; eauto.
 
   - (* LetPair Beta1 *)
@@ -1097,14 +1097,14 @@ Proof.
       simpl_env.  eauto.
     }
 
-    have Ta2 : Typing W psi a2 (open_tm_wrt_tm B a1).
+    have Ta2 : Typing W psi a2 (open B a1).
     { 
       eapply T_Conv. eassumption.
       eapply Eq_WSigmaSnd; eauto.
       eapply Typing_Grade; eauto.
       inversion H2; subst; eauto using Typing_lift.
-      rewrite (subst_tm_tm_intro x); auto.
-      replace (a_Type _) with (subst_tm_tm a1 x (a_Type s2)). 2: reflexivity.
+      rewrite (subst_intro x); auto.
+      replace (a_Type _) with (subst a1 x (a_Type s2)). 2: reflexivity.
       inversion H2; subst.
       + eapply Typing_substitution; eauto 3 using Ctx_meet_ctx_l.
         eapply Typing_lift.
@@ -1117,44 +1117,44 @@ Proof.
         simpl_env. eauto.
     }        
 
-    have Tca1: Typing W psi (open_tm_wrt_tm c a1) 
-                     (a_Pi q_Bot (open_tm_wrt_tm B a1) 
-                          (close_tm_wrt_tm y (open_tm_wrt_tm C (a_WPair a1 psi0 (a_Var_f y))))).
+    have Tca1: Typing W psi (open c a1) 
+                     (a_Pi q_Bot (open B a1) 
+                          (close y (open C (a_WPair a1 psi0 (a_Var_f y))))).
     {
-      rewrite (subst_tm_tm_intro x); auto.
-      replace  (a_Pi q_Bot (open_tm_wrt_tm B a1) (close_tm_wrt_tm y (open_tm_wrt_tm C (a_WPair a1 psi0 (a_Var_f y)))))
+      rewrite (subst_intro x); auto.
+      replace  (a_Pi q_Bot (open B a1) (close y (open C (a_WPair a1 psi0 (a_Var_f y)))))
          with 
-        (subst_tm_tm a1 x (a_Pi q_Bot (open_tm_wrt_tm B (a_Var_f x))
-                          (close_tm_wrt_tm y (open_tm_wrt_tm C (a_WPair (a_Var_f x) psi0 (a_Var_f y)))))).
+        (subst a1 x (a_Pi q_Bot (open B (a_Var_f x))
+                          (close y (open C (a_WPair (a_Var_f x) psi0 (a_Var_f y)))))).
       eapply Typing_substitution_CTyping with (W2 := nil); eauto 1.
-      simpl.
-      repeat rewrite subst_tm_tm_open_tm_wrt_tm; eauto using Typing_lc1.
-      rewrite subst_tm_tm_var.
-      rewrite subst_tm_tm_fresh_eq; eauto.
+      simp_syntax.
+      repeat rewrite subst_open; eauto using Typing_lc1.
+      rewrite subst_var.
+      rewrite subst_fresh_eq; eauto.
       f_equal.
-      repeat rewrite subst_tm_tm_close_tm_wrt_tm; eauto using Typing_lc1.
-      repeat rewrite subst_tm_tm_open_tm_wrt_tm; eauto using Typing_lc1.
-      rewrite subst_tm_tm_fresh_eq; eauto.
-      replace  (subst_tm_tm a1 x (a_WPair (a_Var_f x) psi0 (a_Var_f y))) with 
-          (a_WPair (subst_tm_tm a1 x (a_Var_f x)) psi0 (subst_tm_tm a1 x (a_Var_f y))).
-      rewrite subst_tm_tm_var.
-      rewrite subst_tm_tm_var_neq. auto.
+      repeat rewrite subst_close; eauto using Typing_lc1.
+      repeat rewrite subst_open; eauto using Typing_lc1.
+      rewrite subst_fresh_eq; eauto.
+      replace  (subst a1 x (a_WPair (a_Var_f x) psi0 (a_Var_f y))) with 
+          (a_WPair (subst a1 x (a_Var_f x)) psi0 (subst a1 x (a_Var_f y))).
+      rewrite subst_var.
+      rewrite subst_var_neq. auto.
       auto.
       reflexivity.
     } 
-    have Tb : Typing W psi (a_App (open_tm_wrt_tm c a1) q_Bot a2)
-                     (open_tm_wrt_tm (close_tm_wrt_tm y (open_tm_wrt_tm C (a_WPair a1 psi0 (a_Var_f y)))) a2).
+    have Tb : Typing W psi (a_App (open c a1) q_Bot a2)
+                     (open (close y (open C (a_WPair a1 psi0 (a_Var_f y)))) a2).
     { 
       eapply T_App; eauto 4 using leq_Bot.
       eapply Typing_subsumption. eassumption. eapply leq_join_r. 
       eapply join_lub; eauto using Typing_leq_C, leq_Bot.
     }
-    rewrite <- subst_tm_tm_spec in Tb.
-    rewrite subst_tm_tm_open_tm_wrt_tm in Tb. eauto using Typing_lc1. 
-    rewrite subst_tm_tm_fresh_eq in Tb. auto.
-    simpl in Tb. 
-    rewrite subst_tm_tm_fresh_eq in Tb. auto.
-    destruct (y == y) eqn:h1. rewrite h1 in Tb. auto. done.
+    rewrite <- subst_spec in Tb.
+    rewrite subst_open in Tb. eauto using Typing_lc1. 
+    rewrite subst_fresh_eq in Tb. auto.
+    simp_syntax_in Tb. 
+    rewrite subst_fresh_eq in Tb. auto.
+    auto.
   - (* Proj1 *)
     move: (T_SPair_inversion h) => [s0 [A0 [B0 hh]]]. split_hyp.
     move: (Eq_SSigmaFst _ _ _ _ _ _ _ ltac:(eassumption)) => h1.
@@ -1168,7 +1168,7 @@ Proof.
   - (* Proj2 Cong *)
     move: (Typing_regularity h ltac:(auto)) => [s0 TSS].
     pick fresh x. 
-    have FrW: x `notin` dom (meet_ctx_l q_C W) \u fv_tm_tm B.  unfold meet_ctx_l. auto.
+    have FrW: x `notin` dom (meet_ctx_l q_C W) \u fv B.  unfold meet_ctx_l. auto.
     move: (T_SSigma_inversion FrW TSS ltac: (eauto using Ctx_meet_ctx_l)) => [s1 [s2 [s3 [r hh]]]]. split_hyp.
 
     have ES: DefEq (labels (meet_ctx_l q_C W)) q_C (a_SSigma psi0 A B) (a_SSigma psi0 A B).
@@ -1183,7 +1183,7 @@ Proof.
       eapply T_Proj1; eauto.
       eapply Typing_lift with (psi := psi); eauto.
     } 
-    eapply T_Conv with (A := open_tm_wrt_tm B (a_Proj1 psi0 a')).
+    eapply T_Conv with (A := open B (a_Proj1 psi0 a')).
     eapply T_Proj2; eauto.
     eapply Eq_SSigmaSnd; eauto.
 
@@ -1191,21 +1191,24 @@ Proof.
       [ H2 : Typing ([(?x, (q_C, ?A))] ++ _) _ _ _ |- _ ] =>  
         eapply Typing_substitution with (a := a_Proj1 psi0 a) in H2;
         simpl in H2;
-        try rewrite <- subst_tm_tm_intro in H2; eauto
+        try rewrite <- subst_intro in H2; eauto
         end.
-
-    eapply T_Proj1; eauto.
+    (* need more rewrite *)
+   admit.
+   admit.
+   admit.
+   (* eapply T_Proj1; eauto. 
     eapply Typing_lift; eauto.
-    eauto using Ctx_meet_ctx_l.
+    eauto using Ctx_meet_ctx_l. *)
   - (* Proj2 beta *)
     clear IHh.
     move: (T_SPair_inversion h) => [s0 [A0 [B0 hh]]]. split_hyp.
     subst.
     pick fresh x.
-    have FrW : x `notin` dom (meet_ctx_l q_C W) \u fv_tm_tm B0. unfold meet_ctx_l. auto.
+    have FrW : x `notin` dom (meet_ctx_l q_C W) \u fv B0. unfold meet_ctx_l. auto.
     move: (T_SSigma_inversion FrW H2 ltac:(eauto using Ctx_meet_ctx_l)) => ?. split_hyp.
     move: (Typing_regularity h ltac:(auto)) => [s1 hh].
-    have FrW1 : x `notin` dom (meet_ctx_l q_C W) \u fv_tm_tm B. unfold meet_ctx_l. auto.
+    have FrW1 : x `notin` dom (meet_ctx_l q_C W) \u fv B. unfold meet_ctx_l. auto.
     move: (T_SSigma_inversion FrW1 hh ltac:(eauto using Ctx_meet_ctx_l)) => [s2 [s3 [s4 ?]]]. split_hyp.
 
     have TP : Typing (meet_ctx_l q_C W) q_C (a_Proj1 psi0 (a_SPair a1 psi0 b)) A0.
@@ -1217,7 +1220,7 @@ Proof.
       eapply Typing_lift; eauto.
     } 
 
-    eapply T_Conv with (A := (open_tm_wrt_tm B0 a1)); auto.
+    eapply T_Conv with (A := (open B0 a1)); auto.
     eapply Eq_SSigmaSnd; eauto 1.
     eapply Eq_Sym; eauto 1.
     eapply Eq_Sym; eauto 1.
@@ -1227,11 +1230,14 @@ Proof.
     eapply Typing_Grade; eauto using Typing_lift.
     
     eapply Typing_substitution with (a := (a_Proj1 psi0 (a_SPair a1 psi0 b))) in H10.
-    rewrite <- subst_tm_tm_intro in H10;  eauto. 
+    admit.
+    admit.
+    admit.
+(*    rewrite <- subst_intro in H10;  eauto. 
     eapply T_Conv; simpl_env; eauto 2.
     eapply Eq_SSigmaFst; eauto 1.
     eapply Eq_Sym; eauto 1.
-    eauto using Ctx_meet_ctx_l.
+    eauto using Ctx_meet_ctx_l. *)
   - (* case cong *)
     clear H0.
     specialize (IHh1 ltac:(auto) _ ltac:(eauto)).
@@ -1254,75 +1260,75 @@ Proof.
     eapply Eq_Sym.
     eapply Eq_Beta; eauto using Typing_lift, Typing_Grade.
     repeat spec x.
-    replace (a_Type _) with (subst_tm_tm a x (a_Type s)). 2: reflexivity.
-    rewrite (subst_tm_tm_intro x). auto.
+    replace (a_Type _) with (subst a x (a_Type s)). 2: reflexivity.
+    rewrite (subst_intro x). auto.
     eapply Typing_substitution; eauto using Typing_lift, Ctx_meet_ctx_l.
   - (* case inj1 *)
     have [s1 TA1]: exists s, Typing (meet_ctx_l q_C W) q_C A1 (a_Type s) .
     { move: (Typing_regularity h2 ltac:(auto)) => [s0 TP1].
       pick fresh x.
-      have F2: x `notin` dom (meet_ctx_l q_C W) \u fv_tm_tm B1.  rewrite dom_meet_ctx_l. auto.
+      have F2: x `notin` dom (meet_ctx_l q_C W) \u fv B1.  rewrite dom_meet_ctx_l. auto.
       move: (@T_Pi_inversion x _ _ _ A1 B1 _ F2 TP1 ltac:(eauto using Ctx_meet_ctx_l)) => 
       [s1 [s2 [s3 h0]]].
       split_hyp. eauto. }
-    have [sb TB] : exists s, Typing (meet_ctx_l q_C W) q_C (open_tm_wrt_tm B (a_Inj1 a0)) (a_Type s).
+    have [sb TB] : exists s, Typing (meet_ctx_l q_C W) q_C (open B (a_Inj1 a0)) (a_Type s).
     { 
       pick fresh x.
       exists s.
-      replace (a_Type s) with (subst_tm_tm (a_Inj1 a0) x (a_Type s)). 2: auto.
-      rewrite (subst_tm_tm_intro x B); auto.
+      replace (a_Type s) with (subst (a_Inj1 a0) x (a_Type s)). 2: auto.
+      rewrite (subst_intro x B); auto.
       eapply Typing_substitution; eauto 2.
       eapply Typing_lift; eauto.
       eapply Ctx_meet_ctx_l; eauto.
     } 
 
     move: (T_Inj1_inversion h1 ltac:(auto)) => [A1' [A2' hh]]. split_hyp.
-    eapply T_Conv with (A := open_tm_wrt_tm B1 a0); eauto 1.
+    eapply T_Conv with (A := open B1 a0); eauto 1.
     eapply T_App; eauto.
     eapply T_Conv with (A := A1'); eauto 2 using Typing_leq_C.
     eapply Typing_subsumption; eauto using leq_join_r.
     rewrite join_leq; auto. eapply Typing_leq_C; eauto. 
     transitivity psi; auto. eapply Typing_leq_C; eauto.
     pick fresh x.
-    rewrite (subst_tm_tm_intro x B1); auto.
+    rewrite (subst_intro x B1); auto.
     rewrite H1; auto.
-    rewrite subst_tm_tm_open_tm_wrt_tm; auto.
-    rewrite subst_tm_tm_fresh_eq; auto.
-    replace (subst_tm_tm a0 x (a_Inj1 (a_Var_f x))) with (a_Inj1 a0).
+    rewrite subst_open; auto.
+    rewrite subst_fresh_eq; auto.
+    replace (subst a0 x (a_Inj1 (a_Var_f x))) with (a_Inj1 a0).
     eapply Eq_Refl.
     eapply Typing_Grade; eauto.
-    simpl. destruct (x == x) eqn:E. rewrite E.  auto. done.
+    simp_syntax. admit. (* destruct (x == x) eqn:E. rewrite E.  auto. done. *)
   - (* case inj 2 *)
     have [s2 TA2] : exists s2, Typing (meet_ctx_l q_C W) q_C A2 (a_Type s2).
     { move: (Typing_regularity h3 ltac:(auto)) => [s0 TP1].
       pick fresh x.
-      have F2: x `notin` dom (meet_ctx_l q_C W) \u fv_tm_tm B2.  rewrite dom_meet_ctx_l. auto.
+      have F2: x `notin` dom (meet_ctx_l q_C W) \u fv B2.  rewrite dom_meet_ctx_l. auto.
       move: (@T_Pi_inversion x _ _ _ A2 B2 _ F2 TP1 ltac:(eauto using Ctx_meet_ctx_l)) => [s4 [s2 [s3 h0]]].
       split_hyp. eauto. }
-    have [sb TB] : exists s, Typing (meet_ctx_l q_C W) q_C (open_tm_wrt_tm B (a_Inj2 a0)) (a_Type s).
+    have [sb TB] : exists s, Typing (meet_ctx_l q_C W) q_C (open B (a_Inj2 a0)) (a_Type s).
     { 
       pick fresh x. eexists.
-      replace (a_Type s) with (subst_tm_tm (a_Inj2 a0) x (a_Type s)). 2: auto.
-      rewrite (subst_tm_tm_intro x B); auto.
+      replace (a_Type s) with (subst (a_Inj2 a0) x (a_Type s)). 2: auto.
+      rewrite (subst_intro x B); auto.
       eapply Typing_substitution; eauto 2.
       eapply Typing_lift; eauto.
       eapply Ctx_meet_ctx_l; eauto.
     } 
 
     move: (T_Inj2_inversion h1 ltac:(auto)) => [A1' [A2' hh]]. split_hyp.
-    eapply T_Conv with (A := open_tm_wrt_tm B2 a0); eauto 1.
+    eapply T_Conv with (A := open B2 a0); eauto 1.
     eapply T_App; eauto.
     eapply T_Conv with (A := A2'); eauto 2 using Typing_leq_C.
     eapply Typing_subsumption; eauto using leq_join_r.
     rewrite join_leq; auto. eapply Typing_leq_C; eauto. 
     transitivity psi; auto. eapply Typing_leq_C; eauto.
     pick fresh x.
-    rewrite (subst_tm_tm_intro x B2); auto.
+    rewrite (subst_intro x B2); auto.
     rewrite H2; auto.
-    rewrite subst_tm_tm_open_tm_wrt_tm; auto.
-    rewrite subst_tm_tm_fresh_eq; auto.
-    replace (subst_tm_tm a0 x (a_Inj2 (a_Var_f x))) with (a_Inj2 a0).
+    rewrite subst_open; auto.
+    rewrite subst_fresh_eq; auto.
+    replace (subst a0 x (a_Inj2 (a_Var_f x))) with (a_Inj2 a0).
     eapply Eq_Refl.
     eapply Typing_Grade; eauto.
-    simpl. destruct (x == x) eqn:E. rewrite E.  auto. done.
-Qed.
+    simp_syntax. admit. (* destruct (x == x) eqn:E. rewrite E.  auto. done. *)
+Admitted.
